<?xml version="1.0"?>
<rdf:RDF xmlns="http://emmc.info/emmo#"
     xml:base="http://emmc.info/emmo"
     xmlns:emmo-granularity="http://emmc.info/emmo-granularity#"
     xmlns:rdf="http://www.w3.org/1999/02/22-rdf-syntax-ns#"
     xmlns:owl="http://www.w3.org/2002/07/owl#"
     xmlns:xml="http://www.w3.org/XML/1998/namespace"
     xmlns:xsd="http://www.w3.org/2001/XMLSchema#"
     xmlns:rdfs="http://www.w3.org/2000/01/rdf-schema#"
     xmlns:emmo-core="http://emmc.info/emmo-core#">
    <owl:Ontology rdf:about="http://emmc.info/emmo">
        <owl:versionIRI rdf:resource="http://emmc.info/0.9.10/emmo"/>
        <owl:versionInfo>The European Materials Modelling Ontology

Version 0.9.10</owl:versionInfo>
        <emmo-core:EMMO_cd5fb112_7ee7_4120_a35d_3ca3e6c3f4ab>Emanuele Ghedini (University of Bologna, IT)
Gerhard Goldbeck (GCL Ltd, UK)
Adham Hashibon (Fraunhofer IWM, DE)
Georg Schmitz (Access, DE)
Jesper Friis (SINTEF, NO)</emmo-core:EMMO_cd5fb112_7ee7_4120_a35d_3ca3e6c3f4ab>
        <rdfs:comment>The emmo-4d module includes the parthood relations that distinguish between partitioning in 3D space and 1D time dimensions.
It depends on emmo-core which is valid for generic topological spaces without a specific dimensionality.</rdfs:comment>
        <emmo-core:EMMO_5525a055_dda5_4556_8b91_f0d22fa676cc>EMMO is released under a Creative Commons license Attribution 4.0 International (CC BY 4.0)

https://creativecommons.org/licenses/by/4.0/legalcode</emmo-core:EMMO_5525a055_dda5_4556_8b91_f0d22fa676cc>
        <rdfs:comment>Contacts:
Gerhard Goldbeck
Goldbeck Consulting Ltd (UK)
email: gerhard@goldbeck-consulting.com

Emanuele Ghedini
University of Bologna (IT)
email: emanuele.ghedini@unibo.it</rdfs:comment>
        <rdfs:comment>The emmo-core module provide the fundamental axioms to express real world obejcts in an a-tomistic mereotpological framework, introducing the distinction between items and collections, and the fundamental mereotopological relations.</rdfs:comment>
        <rdfs:comment>The EMMO requires FacT++ reasoner plugin in order to visualize all inferences and class hierarchy (ctrl+R hotkey in Protege).</rdfs:comment>
        <rdfs:comment>The EMMO requires FaCT++ reasoner plugin in order to visualize all inferences and class hierarchy (ctrl+R hotkey in Protege).</rdfs:comment>
        <rdfs:comment>European Materials and Modelling Ontology (EMMO)

EMMO is a multidisciplinary effort to develop a standard representational framework (the ontology) based on current materials modelling knowledge, including physical sciences, analytical philosophy and information and communication technologies. 

It provides the connection between the physical world, materials characterisation world and materials modelling world.</rdfs:comment>
    </owl:Ontology>
    


    <!-- 
    ///////////////////////////////////////////////////////////////////////////////////////
    //
    // Annotation properties
    //
    ///////////////////////////////////////////////////////////////////////////////////////
     -->

    


    <!-- http://emmc.info/emmo-core#EMMO_5525a055_dda5_4556_8b91_f0d22fa676cc -->

    <rdf:Description rdf:about="http://emmc.info/emmo-core#EMMO_5525a055_dda5_4556_8b91_f0d22fa676cc">
        <rdfs:label xml:lang="en">license</rdfs:label>
    </rdf:Description>
    


    <!-- http://emmc.info/emmo-core#EMMO_70fe84ff_99b6_4206_a9fc_9a8931836d84 -->

    <owl:AnnotationProperty rdf:about="http://emmc.info/emmo-core#EMMO_70fe84ff_99b6_4206_a9fc_9a8931836d84">
        <rdfs:label xml:lang="en">definition</rdfs:label>
    </owl:AnnotationProperty>
    


    <!-- http://emmc.info/emmo-core#EMMO_967080e5_2f42_4eb2_a3a9_c58143e835f9 -->

    <owl:AnnotationProperty rdf:about="http://emmc.info/emmo-core#EMMO_967080e5_2f42_4eb2_a3a9_c58143e835f9">
        <rdfs:label xml:lang="en">elucidation</rdfs:label>
    </owl:AnnotationProperty>
    


    <!-- http://emmc.info/emmo-core#EMMO_b432d2d5_25f4_4165_99c5_5935a7763c1a -->

    <owl:AnnotationProperty rdf:about="http://emmc.info/emmo-core#EMMO_b432d2d5_25f4_4165_99c5_5935a7763c1a">
        <rdfs:label xml:lang="en">example</rdfs:label>
    </owl:AnnotationProperty>
    


    <!-- http://emmc.info/emmo-core#EMMO_cd5fb112_7ee7_4120_a35d_3ca3e6c3f4ab -->

    <rdf:Description rdf:about="http://emmc.info/emmo-core#EMMO_cd5fb112_7ee7_4120_a35d_3ca3e6c3f4ab">
        <rdfs:label xml:lang="en">author</rdfs:label>
    </rdf:Description>
    


    <!-- 
    ///////////////////////////////////////////////////////////////////////////////////////
    //
    // Object Properties
    //
    ///////////////////////////////////////////////////////////////////////////////////////
     -->

    


    <!-- http://emmc.info/emmo-4d#EMMO_6e046dd0_9634_4013_b2b1_9cc468087c83 -->

    <owl:ObjectProperty rdf:about="http://emmc.info/emmo-4d#EMMO_6e046dd0_9634_4013_b2b1_9cc468087c83">
        <rdfs:subPropertyOf rdf:resource="http://emmc.info/emmo-core#EMMO_9380ab64_0363_4804_b13f_3a8a94119a76"/>
        <rdf:type rdf:resource="http://www.w3.org/2002/07/owl#TransitiveProperty"/>
        <rdfs:domain rdf:resource="http://emmc.info/emmo-core#EMMO_eb3a768e_d53e_4be9_a23b_0714833c36de"/>
        <rdfs:range rdf:resource="http://emmc.info/emmo-core#EMMO_eb3a768e_d53e_4be9_a23b_0714833c36de"/>
        <emmo-core:EMMO_967080e5_2f42_4eb2_a3a9_c58143e835f9>A relation that isolates a proper part that extends itself in time through a portion of the lifetime whole.</emmo-core:EMMO_967080e5_2f42_4eb2_a3a9_c58143e835f9>
        <rdfs:label xml:lang="en">has_spatio-temporal_part</rdfs:label>
    </owl:ObjectProperty>
    


    <!-- http://emmc.info/emmo-4d#EMMO_f68030be_94b8_4c61_a161_886468558054 -->

    <owl:ObjectProperty rdf:about="http://emmc.info/emmo-4d#EMMO_f68030be_94b8_4c61_a161_886468558054">
        <rdfs:subPropertyOf rdf:resource="http://emmc.info/emmo-core#EMMO_9380ab64_0363_4804_b13f_3a8a94119a76"/>
        <rdf:type rdf:resource="http://www.w3.org/2002/07/owl#TransitiveProperty"/>
        <rdfs:domain rdf:resource="http://emmc.info/emmo-core#EMMO_eb3a768e_d53e_4be9_a23b_0714833c36de"/>
        <rdfs:range rdf:resource="http://emmc.info/emmo-core#EMMO_eb3a768e_d53e_4be9_a23b_0714833c36de"/>
        <emmo-core:EMMO_967080e5_2f42_4eb2_a3a9_c58143e835f9>A relation that isolates a proper part that extends itself in time within the lifetime of the whole, without covering the full spatial extension of the 4D whole (i.e. is not a temporal part).</emmo-core:EMMO_967080e5_2f42_4eb2_a3a9_c58143e835f9>
        <rdfs:label xml:lang="en">has_spatial_part</rdfs:label>
    </owl:ObjectProperty>
    


    <!-- http://emmc.info/emmo-core#EMMO_03212fd7_abfd_4828_9c8e_62c293052d4b -->

    <owl:ObjectProperty rdf:about="http://emmc.info/emmo-core#EMMO_03212fd7_abfd_4828_9c8e_62c293052d4b">
        <rdfs:subPropertyOf rdf:resource="http://emmc.info/emmo-core#EMMO_ec2472ae_cf4a_46a5_8555_1556f5a6c3c5"/>
        <emmo-core:EMMO_967080e5_2f42_4eb2_a3a9_c58143e835f9>The generic EMMO mereotopological relation.</emmo-core:EMMO_967080e5_2f42_4eb2_a3a9_c58143e835f9>
        <rdfs:comment>Mereotopology merges mereological and topological concepts and provides relations between wholes, parts, boundaries, etc.</rdfs:comment>
        <rdfs:label xml:lang="en">mereotopological</rdfs:label>
    </owl:ObjectProperty>
    


    <!-- http://emmc.info/emmo-core#EMMO_17e27c22_37e1_468c_9dd7_95e137f73e7f -->

    <owl:ObjectProperty rdf:about="http://emmc.info/emmo-core#EMMO_17e27c22_37e1_468c_9dd7_95e137f73e7f">
        <rdfs:subPropertyOf rdf:resource="http://emmc.info/emmo-core#EMMO_8c898653_1118_4682_9bbf_6cc334d16a99"/>
        <rdfs:subPropertyOf rdf:resource="http://emmc.info/emmo-core#EMMO_d893d373_b579_4867_841e_1c2b31a8d2c6"/>
        <rdfs:subPropertyOf>
            <rdf:Description>
                <owl:inverseOf rdf:resource="http://emmc.info/emmo-core#EMMO_d893d373_b579_4867_841e_1c2b31a8d2c6"/>
            </rdf:Description>
        </rdfs:subPropertyOf>
        <rdf:type rdf:resource="http://www.w3.org/2002/07/owl#TransitiveProperty"/>
        <emmo-core:EMMO_967080e5_2f42_4eb2_a3a9_c58143e835f9>The primitive relation of parthood (reflexive, transitive, antisymmetric).

Pxy ≡ x is part of y</emmo-core:EMMO_967080e5_2f42_4eb2_a3a9_c58143e835f9>
        <rdfs:label xml:lang="en">has_part</rdfs:label>
        <rdfs:seeAlso>is_part_of</rdfs:seeAlso>
    </owl:ObjectProperty>
    


    <!-- http://emmc.info/emmo-core#EMMO_4d6504f1_c470_4ce9_b941_bbbebc9ab05d -->

    <owl:ObjectProperty rdf:about="http://emmc.info/emmo-core#EMMO_4d6504f1_c470_4ce9_b941_bbbebc9ab05d">
        <rdfs:subPropertyOf rdf:resource="http://emmc.info/emmo-core#EMMO_6703954e_34c4_4a15_a9e7_f313760ae1a8"/>
        <rdfs:subPropertyOf>
            <rdf:Description>
                <owl:inverseOf rdf:resource="http://emmc.info/emmo-core#EMMO_6703954e_34c4_4a15_a9e7_f313760ae1a8"/>
            </rdf:Description>
        </rdfs:subPropertyOf>
        <owl:inverseOf rdf:resource="http://emmc.info/emmo-core#EMMO_4d6504f1_c470_4ce9_b941_bbbebc9ab05d"/>
        <rdf:type rdf:resource="http://www.w3.org/2002/07/owl#SymmetricProperty"/>
        <emmo-core:EMMO_70fe84ff_99b6_4206_a9fc_9a8931836d84>ECxy ≡ Cxy ∧ ¬Oxy</emmo-core:EMMO_70fe84ff_99b6_4206_a9fc_9a8931836d84>
        <emmo-core:EMMO_967080e5_2f42_4eb2_a3a9_c58143e835f9>The relation between two connected but not overlapping real world objects, also known as external connection</emmo-core:EMMO_967080e5_2f42_4eb2_a3a9_c58143e835f9>
        <rdfs:label xml:lang="en">contacts</rdfs:label>
    </owl:ObjectProperty>
    


    <!-- http://emmc.info/emmo-core#EMMO_517dfaf9_4970_41ac_81ee_d031627d2c7c -->

    <owl:ObjectProperty rdf:about="http://emmc.info/emmo-core#EMMO_517dfaf9_4970_41ac_81ee_d031627d2c7c">
        <rdfs:subPropertyOf rdf:resource="http://emmc.info/emmo-core#EMMO_03212fd7_abfd_4828_9c8e_62c293052d4b"/>
        <rdfs:subPropertyOf>
            <rdf:Description>
                <owl:inverseOf rdf:resource="http://emmc.info/emmo-core#EMMO_03212fd7_abfd_4828_9c8e_62c293052d4b"/>
            </rdf:Description>
        </rdfs:subPropertyOf>
        <owl:inverseOf rdf:resource="http://emmc.info/emmo-core#EMMO_517dfaf9_4970_41ac_81ee_d031627d2c7c"/>
        <rdf:type rdf:resource="http://www.w3.org/2002/07/owl#SymmetricProperty"/>
        <emmo-core:EMMO_967080e5_2f42_4eb2_a3a9_c58143e835f9>The relation between two individuals that stand for real world topological disconnected objects.</emmo-core:EMMO_967080e5_2f42_4eb2_a3a9_c58143e835f9>
        <rdfs:label xml:lang="en">disconnected</rdfs:label>
    </owl:ObjectProperty>
    


    <!-- http://emmc.info/emmo-core#EMMO_6703954e_34c4_4a15_a9e7_f313760ae1a8 -->

    <owl:ObjectProperty rdf:about="http://emmc.info/emmo-core#EMMO_6703954e_34c4_4a15_a9e7_f313760ae1a8">
        <rdfs:subPropertyOf rdf:resource="http://emmc.info/emmo-core#EMMO_03212fd7_abfd_4828_9c8e_62c293052d4b"/>
        <rdfs:subPropertyOf>
            <rdf:Description>
                <owl:inverseOf rdf:resource="http://emmc.info/emmo-core#EMMO_03212fd7_abfd_4828_9c8e_62c293052d4b"/>
            </rdf:Description>
        </rdfs:subPropertyOf>
        <owl:inverseOf rdf:resource="http://emmc.info/emmo-core#EMMO_6703954e_34c4_4a15_a9e7_f313760ae1a8"/>
        <rdf:type rdf:resource="http://www.w3.org/2002/07/owl#SymmetricProperty"/>
        <emmo-core:EMMO_70fe84ff_99b6_4206_a9fc_9a8931836d84>Definition:
Cxy ≡ x is connected with y

Axiom:
 1) Cxx (x is always connected with itself (reflexivity))
Axiom:
2) Cxy → Cyx (if x is connected with y then y is connected with x (symmetry))</emmo-core:EMMO_70fe84ff_99b6_4206_a9fc_9a8931836d84>
        <emmo-core:EMMO_967080e5_2f42_4eb2_a3a9_c58143e835f9>The relation between two individuals that stand for real world topological connected objects.</emmo-core:EMMO_967080e5_2f42_4eb2_a3a9_c58143e835f9>
        <rdfs:comment>Causality is a topological property between connected items.</rdfs:comment>
        <rdfs:comment>Items being connected means that there is a topological contact or &quot;interaction&quot; between them.</rdfs:comment>
        <rdfs:label xml:lang="en">connected</rdfs:label>
    </owl:ObjectProperty>
    


    <!-- http://emmc.info/emmo-core#EMMO_6b7276a4_4b9d_440a_b577_0277539c0fc4 -->

    <owl:ObjectProperty rdf:about="http://emmc.info/emmo-core#EMMO_6b7276a4_4b9d_440a_b577_0277539c0fc4">
        <rdfs:subPropertyOf rdf:resource="http://emmc.info/emmo-core#EMMO_9380ab64_0363_4804_b13f_3a8a94119a76"/>
        <rdf:type rdf:resource="http://www.w3.org/2002/07/owl#AsymmetricProperty"/>
        <rdf:type rdf:resource="http://www.w3.org/2002/07/owl#IrreflexiveProperty"/>
        <rdfs:domain rdf:resource="http://emmc.info/emmo-core#EMMO_2d2ecd97_067f_4d0e_950c_d746b7700a31"/>
        <rdfs:range rdf:resource="http://emmc.info/emmo-core#EMMO_eb3a768e_d53e_4be9_a23b_0714833c36de"/>
        <emmo-core:EMMO_967080e5_2f42_4eb2_a3a9_c58143e835f9>The relation that connects and individual that stands for a collection to an individual that stands for a member of the collections.

A member is a proper part of the collection that:
- is an item (i.e. is a self-connected object)
- is maximally self-connected with respect to the collection (i.e. it is not in contact with other members of the same collection)</emmo-core:EMMO_967080e5_2f42_4eb2_a3a9_c58143e835f9>
        <rdfs:label xml:lang="en">has_member</rdfs:label>
    </owl:ObjectProperty>
    


    <!-- http://emmc.info/emmo-core#EMMO_7afbed84_7593_4a23_bd88_9d9c6b04e8f6 -->

    <owl:ObjectProperty rdf:about="http://emmc.info/emmo-core#EMMO_7afbed84_7593_4a23_bd88_9d9c6b04e8f6">
        <rdfs:subPropertyOf rdf:resource="http://emmc.info/emmo-core#EMMO_9380ab64_0363_4804_b13f_3a8a94119a76"/>
        <rdf:type rdf:resource="http://www.w3.org/2002/07/owl#TransitiveProperty"/>
        <rdfs:domain rdf:resource="http://emmc.info/emmo-core#EMMO_eb3a768e_d53e_4be9_a23b_0714833c36de"/>
        <rdfs:range rdf:resource="http://emmc.info/emmo-core#EMMO_eb3a768e_d53e_4be9_a23b_0714833c36de"/>
        <emmo-core:EMMO_967080e5_2f42_4eb2_a3a9_c58143e835f9>A relation that isolate a proper part that covers the total spatial extension of a whole within a time interval.</emmo-core:EMMO_967080e5_2f42_4eb2_a3a9_c58143e835f9>
        <rdfs:label xml:lang="en">has_temporal_part</rdfs:label>
    </owl:ObjectProperty>
    


    <!-- http://emmc.info/emmo-core#EMMO_8c898653_1118_4682_9bbf_6cc334d16a99 -->

    <owl:ObjectProperty rdf:about="http://emmc.info/emmo-core#EMMO_8c898653_1118_4682_9bbf_6cc334d16a99">
        <rdfs:subPropertyOf rdf:resource="http://emmc.info/emmo-core#EMMO_6703954e_34c4_4a15_a9e7_f313760ae1a8"/>
        <rdfs:subPropertyOf>
            <rdf:Description>
                <owl:inverseOf rdf:resource="http://emmc.info/emmo-core#EMMO_6703954e_34c4_4a15_a9e7_f313760ae1a8"/>
            </rdf:Description>
        </rdfs:subPropertyOf>
        <rdf:type rdf:resource="http://www.w3.org/2002/07/owl#TransitiveProperty"/>
        <emmo-core:EMMO_70fe84ff_99b6_4206_a9fc_9a8931836d84>Exy ≡ ∀z(Czx → Czy)</emmo-core:EMMO_70fe84ff_99b6_4206_a9fc_9a8931836d84>
        <rdfs:comment>Enclosure is reflexive and transitive.</rdfs:comment>
        <rdfs:label xml:lang="en">encloses</rdfs:label>
        <rdfs:seeAlso>is_enclosed_by</rdfs:seeAlso>
    </owl:ObjectProperty>
    


    <!-- http://emmc.info/emmo-core#EMMO_9380ab64_0363_4804_b13f_3a8a94119a76 -->

    <owl:ObjectProperty rdf:about="http://emmc.info/emmo-core#EMMO_9380ab64_0363_4804_b13f_3a8a94119a76">
        <rdfs:subPropertyOf rdf:resource="http://emmc.info/emmo-core#EMMO_17e27c22_37e1_468c_9dd7_95e137f73e7f"/>
        <rdf:type rdf:resource="http://www.w3.org/2002/07/owl#TransitiveProperty"/>
        <emmo-core:EMMO_70fe84ff_99b6_4206_a9fc_9a8931836d84>PPxy ≡ Pxy ∧ ¬(x=y)</emmo-core:EMMO_70fe84ff_99b6_4206_a9fc_9a8931836d84>
        <rdfs:label xml:lang="en">has_proper_part</rdfs:label>
        <rdfs:seeAlso>is_proper_part_of</rdfs:seeAlso>
    </owl:ObjectProperty>
    


    <!-- http://emmc.info/emmo-core#EMMO_9cb984ca_48ad_4864_b09e_50d3fff19420 -->

    <owl:ObjectProperty rdf:about="http://emmc.info/emmo-core#EMMO_9cb984ca_48ad_4864_b09e_50d3fff19420">
        <rdfs:subPropertyOf rdf:resource="http://emmc.info/emmo-core#EMMO_d893d373_b579_4867_841e_1c2b31a8d2c6"/>
        <rdfs:subPropertyOf>
            <rdf:Description>
                <owl:inverseOf rdf:resource="http://emmc.info/emmo-core#EMMO_d893d373_b579_4867_841e_1c2b31a8d2c6"/>
            </rdf:Description>
        </rdfs:subPropertyOf>
        <owl:inverseOf rdf:resource="http://emmc.info/emmo-core#EMMO_9cb984ca_48ad_4864_b09e_50d3fff19420"/>
        <rdf:type rdf:resource="http://www.w3.org/2002/07/owl#SymmetricProperty"/>
        <emmo-core:EMMO_967080e5_2f42_4eb2_a3a9_c58143e835f9>A relation between two overlapping real world objects without one being part of the other.</emmo-core:EMMO_967080e5_2f42_4eb2_a3a9_c58143e835f9>
        <rdfs:label xml:lang="en">overcrosses</rdfs:label>
    </owl:ObjectProperty>
    


    <!-- http://emmc.info/emmo-core#EMMO_d893d373_b579_4867_841e_1c2b31a8d2c6 -->

    <owl:ObjectProperty rdf:about="http://emmc.info/emmo-core#EMMO_d893d373_b579_4867_841e_1c2b31a8d2c6">
        <rdfs:subPropertyOf rdf:resource="http://emmc.info/emmo-core#EMMO_6703954e_34c4_4a15_a9e7_f313760ae1a8"/>
        <rdfs:subPropertyOf>
            <rdf:Description>
                <owl:inverseOf rdf:resource="http://emmc.info/emmo-core#EMMO_6703954e_34c4_4a15_a9e7_f313760ae1a8"/>
            </rdf:Description>
        </rdfs:subPropertyOf>
        <owl:inverseOf rdf:resource="http://emmc.info/emmo-core#EMMO_d893d373_b579_4867_841e_1c2b31a8d2c6"/>
        <rdf:type rdf:resource="http://www.w3.org/2002/07/owl#SymmetricProperty"/>
        <emmo-core:EMMO_70fe84ff_99b6_4206_a9fc_9a8931836d84>Oxy ≡ ∃z(Pzx ∧ Pzy)

x overlap with y means that there exists a z that is part of both x and y</emmo-core:EMMO_70fe84ff_99b6_4206_a9fc_9a8931836d84>
        <rdfs:label xml:lang="en">overlaps</rdfs:label>
    </owl:ObjectProperty>
    


    <!-- http://emmc.info/emmo-core#EMMO_ec2472ae_cf4a_46a5_8555_1556f5a6c3c5 -->

    <owl:ObjectProperty rdf:about="http://emmc.info/emmo-core#EMMO_ec2472ae_cf4a_46a5_8555_1556f5a6c3c5">
        <rdfs:subPropertyOf rdf:resource="http://www.w3.org/2002/07/owl#topObjectProperty"/>
        <rdfs:domain rdf:resource="http://emmc.info/emmo-core#EMMO_802d3e92_8770_4f98_a289_ccaaab7fdddf"/>
        <rdfs:range rdf:resource="http://emmc.info/emmo-core#EMMO_802d3e92_8770_4f98_a289_ccaaab7fdddf"/>
        <emmo-core:EMMO_967080e5_2f42_4eb2_a3a9_c58143e835f9>The sign that stand for the most generic EMMO relation.</emmo-core:EMMO_967080e5_2f42_4eb2_a3a9_c58143e835f9>
        <rdfs:label xml:lang="en">emmo_relation</rdfs:label>
    </owl:ObjectProperty>
    


    <!-- http://emmc.info/emmo-granularity#EMMO_65a2c5b8_e4d8_4a51_b2f8_e55effc0547d -->

    <owl:ObjectProperty rdf:about="http://emmc.info/emmo-granularity#EMMO_65a2c5b8_e4d8_4a51_b2f8_e55effc0547d">
        <rdfs:subPropertyOf rdf:resource="http://emmc.info/emmo-core#EMMO_7afbed84_7593_4a23_bd88_9d9c6b04e8f6"/>
        <rdf:type rdf:resource="http://www.w3.org/2002/07/owl#InverseFunctionalProperty"/>
        <rdf:type rdf:resource="http://www.w3.org/2002/07/owl#AsymmetricProperty"/>
        <rdf:type rdf:resource="http://www.w3.org/2002/07/owl#IrreflexiveProperty"/>
        <rdfs:domain rdf:resource="http://emmc.info/emmo-granularity#EMMO_52211e5e_d767_4812_845e_eb6b402c476a"/>
        <rdfs:range rdf:resource="http://emmc.info/emmo-granularity#EMMO_36c79456_e29c_400d_8bd3_0eedddb82652"/>
        <rdfs:label xml:lang="en">has_temporal_direct_part</rdfs:label>
    </owl:ObjectProperty>
    


    <!-- http://emmc.info/emmo-granularity#EMMO_a50d920d_1ee3_4668_9a73_5d80a1c6fe15 -->

    <owl:ObjectProperty rdf:about="http://emmc.info/emmo-granularity#EMMO_a50d920d_1ee3_4668_9a73_5d80a1c6fe15">
        <rdfs:subPropertyOf rdf:resource="http://emmc.info/emmo-4d#EMMO_6e046dd0_9634_4013_b2b1_9cc468087c83"/>
        <rdf:type rdf:resource="http://www.w3.org/2002/07/owl#InverseFunctionalProperty"/>
        <rdf:type rdf:resource="http://www.w3.org/2002/07/owl#AsymmetricProperty"/>
        <rdf:type rdf:resource="http://www.w3.org/2002/07/owl#IrreflexiveProperty"/>
        <rdfs:domain rdf:resource="http://emmc.info/emmo-granularity#EMMO_52211e5e_d767_4812_845e_eb6b402c476a"/>
        <rdfs:range rdf:resource="http://emmc.info/emmo-granularity#EMMO_52211e5e_d767_4812_845e_eb6b402c476a"/>
        <rdfs:label xml:lang="en">has_spatio-temporal_direct_part</rdfs:label>
    </owl:ObjectProperty>
    


    <!-- http://emmc.info/emmo-granularity#EMMO_b2282816_b7a3_44c6_b2cb_3feff1ceb7fe -->

    <owl:ObjectProperty rdf:about="http://emmc.info/emmo-granularity#EMMO_b2282816_b7a3_44c6_b2cb_3feff1ceb7fe">
        <rdfs:subPropertyOf rdf:resource="http://emmc.info/emmo-4d#EMMO_f68030be_94b8_4c61_a161_886468558054"/>
        <rdf:type rdf:resource="http://www.w3.org/2002/07/owl#InverseFunctionalProperty"/>
        <rdf:type rdf:resource="http://www.w3.org/2002/07/owl#AsymmetricProperty"/>
        <rdf:type rdf:resource="http://www.w3.org/2002/07/owl#IrreflexiveProperty"/>
        <rdfs:domain rdf:resource="http://emmc.info/emmo-granularity#EMMO_52211e5e_d767_4812_845e_eb6b402c476a"/>
        <rdfs:range rdf:resource="http://emmc.info/emmo-granularity#EMMO_52211e5e_d767_4812_845e_eb6b402c476a"/>
        <rdfs:label xml:lang="en">has_spatial_direct_part</rdfs:label>
    </owl:ObjectProperty>
    


    <!-- http://emmc.info/emmo-process#EMMO_ae2d1a96_bfa1_409a_a7d2_03d69e8a125a -->

    <owl:ObjectProperty rdf:about="http://emmc.info/emmo-process#EMMO_ae2d1a96_bfa1_409a_a7d2_03d69e8a125a">
        <rdfs:subPropertyOf rdf:resource="http://emmc.info/emmo-core#EMMO_17e27c22_37e1_468c_9dd7_95e137f73e7f"/>
        <rdfs:domain rdf:resource="http://emmc.info/emmo-process#EMMO_43e9a05d_98af_41b4_92f6_00f79a09bfce"/>
        <rdfs:range rdf:resource="http://emmc.info/emmo-process#EMMO_49804605_c0fe_4538_abda_f70ba1dc8a5d"/>
        <emmo-core:EMMO_967080e5_2f42_4eb2_a3a9_c58143e835f9>The raltion between a process and an object participating to it.</emmo-core:EMMO_967080e5_2f42_4eb2_a3a9_c58143e835f9>
        <rdfs:comment>Participation is a parthood relation: you must be part (and then be connected) of the process to contribute to it.</rdfs:comment>
        <rdfs:comment>Participation is not under direct parthood since a process is not strictly related to reductionism, but it&apos;s a way to categorize temporal regions by the interpreters.</rdfs:comment>
        <rdfs:label xml:lang="en">has_participant</rdfs:label>
    </owl:ObjectProperty>
    


    <!-- http://emmc.info/emmo-process#EMMO_c5aae418_1622_4d02_93c5_21159e28e6c1 -->

    <owl:ObjectProperty rdf:about="http://emmc.info/emmo-process#EMMO_c5aae418_1622_4d02_93c5_21159e28e6c1">
        <rdfs:subPropertyOf rdf:resource="http://emmc.info/emmo-core#EMMO_9380ab64_0363_4804_b13f_3a8a94119a76"/>
        <rdfs:subPropertyOf rdf:resource="http://emmc.info/emmo-process#EMMO_ae2d1a96_bfa1_409a_a7d2_03d69e8a125a"/>
        <rdfs:label xml:lang="en">has_proper_participant</rdfs:label>
    </owl:ObjectProperty>
    


    <!-- http://emmc.info/emmo-properties#EMMO_e1097637_70d2_4895_973f_2396f04fa204 -->

    <owl:ObjectProperty rdf:about="http://emmc.info/emmo-properties#EMMO_e1097637_70d2_4895_973f_2396f04fa204">
        <rdfs:subPropertyOf rdf:resource="http://emmc.info/emmo-semiotics#EMMO_eb3518bf_f799_4f9e_8c3e_ce59af11453b"/>
        <rdfs:range rdf:resource="http://emmc.info/emmo-properties#EMMO_b7bcff25_ffc3_474e_9ab5_01b1664bd4ba"/>
        <rdfs:label xml:lang="en">has_property</rdfs:label>
    </owl:ObjectProperty>
    


    <!-- http://emmc.info/emmo-semiotics#EMMO_2337e25c_3c60_43fc_a8f9_b11a3f974291 -->

    <owl:ObjectProperty rdf:about="http://emmc.info/emmo-semiotics#EMMO_2337e25c_3c60_43fc_a8f9_b11a3f974291">
        <rdfs:subPropertyOf rdf:resource="http://emmc.info/emmo-core#EMMO_ec2472ae_cf4a_46a5_8555_1556f5a6c3c5"/>
        <emmo-core:EMMO_967080e5_2f42_4eb2_a3a9_c58143e835f9>The generic EMMO semiotical relation.</emmo-core:EMMO_967080e5_2f42_4eb2_a3a9_c58143e835f9>
        <rdfs:label xml:lang="en">semiotical</rdfs:label>
    </owl:ObjectProperty>
    


    <!-- http://emmc.info/emmo-semiotics#EMMO_297999d6_c9e4_4262_9536_bd524d1c6e21 -->

    <owl:ObjectProperty rdf:about="http://emmc.info/emmo-semiotics#EMMO_297999d6_c9e4_4262_9536_bd524d1c6e21">
        <rdfs:subPropertyOf rdf:resource="http://emmc.info/emmo-semiotics#EMMO_60577dea_9019_4537_ac41_80b0fb563d41"/>
        <rdfs:range rdf:resource="http://emmc.info/emmo-semiotics#EMMO_0cd58641_824c_4851_907f_f4c3be76630c"/>
        <rdfs:label xml:lang="en">has_index</rdfs:label>
    </owl:ObjectProperty>
    


    <!-- http://emmc.info/emmo-semiotics#EMMO_39c3815d_8cae_4c8f_b2ff_eeba24bec455 -->

    <owl:ObjectProperty rdf:about="http://emmc.info/emmo-semiotics#EMMO_39c3815d_8cae_4c8f_b2ff_eeba24bec455">
        <rdfs:subPropertyOf rdf:resource="http://emmc.info/emmo-semiotics#EMMO_60577dea_9019_4537_ac41_80b0fb563d41"/>
        <rdfs:range rdf:resource="http://emmc.info/emmo-semiotics#EMMO_d7788d1a_020d_4c78_85a1_13563fcec168"/>
        <rdfs:label xml:lang="en">has_icon</rdfs:label>
    </owl:ObjectProperty>
    


    <!-- http://emmc.info/emmo-semiotics#EMMO_60577dea_9019_4537_ac41_80b0fb563d41 -->

    <owl:ObjectProperty rdf:about="http://emmc.info/emmo-semiotics#EMMO_60577dea_9019_4537_ac41_80b0fb563d41">
        <rdfs:subPropertyOf rdf:resource="http://emmc.info/emmo-semiotics#EMMO_2337e25c_3c60_43fc_a8f9_b11a3f974291"/>
        <rdfs:domain rdf:resource="http://emmc.info/emmo-semiotics#EMMO_6f5af708_f825_4feb_a0d1_a8d813d3022b"/>
        <rdfs:range rdf:resource="http://emmc.info/emmo-semiotics#EMMO_b21a56ed_f969_4612_a6ec_cb7766f7f31d"/>
        <rdfs:label xml:lang="en">has_sign</rdfs:label>
    </owl:ObjectProperty>
    


    <!-- http://emmc.info/emmo-semiotics#EMMO_eb3518bf_f799_4f9e_8c3e_ce59af11453b -->

    <owl:ObjectProperty rdf:about="http://emmc.info/emmo-semiotics#EMMO_eb3518bf_f799_4f9e_8c3e_ce59af11453b">
        <rdfs:subPropertyOf rdf:resource="http://emmc.info/emmo-semiotics#EMMO_60577dea_9019_4537_ac41_80b0fb563d41"/>
        <rdfs:range rdf:resource="http://emmc.info/emmo-semiotics#EMMO_35d2e130_6e01_41ed_94f7_00b333d46cf9"/>
        <rdfs:label xml:lang="en">has_convention</rdfs:label>
    </owl:ObjectProperty>
    


    <!-- http://www.w3.org/2002/07/owl#topObjectProperty -->

    <rdf:Description rdf:about="http://www.w3.org/2002/07/owl#topObjectProperty">
        <owl:inverseOf rdf:resource="http://www.w3.org/2002/07/owl#topObjectProperty"/>
        <rdf:type rdf:resource="http://www.w3.org/2002/07/owl#SymmetricProperty"/>
        <rdf:type rdf:resource="http://www.w3.org/2002/07/owl#TransitiveProperty"/>
        <rdf:type rdf:resource="http://www.w3.org/2002/07/owl#ReflexiveProperty"/>
    </rdf:Description>
    


    <!-- 
    ///////////////////////////////////////////////////////////////////////////////////////
    //
    // Classes
    //
    ///////////////////////////////////////////////////////////////////////////////////////
     -->

    


    <!-- http://emmc.info/emmo-core#EMMO_0f795e3e_c602_4577_9a43_d5a231aa1360 -->

    <owl:Class rdf:about="http://emmc.info/emmo-core#EMMO_0f795e3e_c602_4577_9a43_d5a231aa1360">
        <rdfs:subClassOf rdf:resource="http://emmc.info/emmo-core#EMMO_c5ddfdba_c074_4aa4_ad6b_1ac4942d300d"/>
        <rdfs:subClassOf rdf:resource="http://emmc.info/emmo-granularity#EMMO_36c79456_e29c_400d_8bd3_0eedddb82652"/>
        <rdfs:subClassOf>
            <owl:Restriction>
                <owl:onProperty rdf:resource="http://emmc.info/emmo-4d#EMMO_f68030be_94b8_4c61_a161_886468558054"/>
                <owl:allValuesFrom rdf:resource="http://www.w3.org/2002/07/owl#Nothing"/>
            </owl:Restriction>
        </rdfs:subClassOf>
        <rdfs:subClassOf>
            <owl:Restriction>
                <owl:onProperty rdf:resource="http://emmc.info/emmo-core#EMMO_7afbed84_7593_4a23_bd88_9d9c6b04e8f6"/>
                <owl:allValuesFrom rdf:resource="http://emmc.info/emmo-core#EMMO_0f795e3e_c602_4577_9a43_d5a231aa1360"/>
            </owl:Restriction>
        </rdfs:subClassOf>
        <emmo-core:EMMO_967080e5_2f42_4eb2_a3a9_c58143e835f9>The basic constituent of &apos;item&apos;-s that can be proper partitioned only in time up to quantum level.</emmo-core:EMMO_967080e5_2f42_4eb2_a3a9_c58143e835f9>
        <rdfs:comment>&apos;elementary&apos; is by definition the most simple example of &apos;state&apos;.</rdfs:comment>
        <rdfs:comment>According to mereology, this should be call &apos;a-tomistic&apos; in the strict etimological sense of the word (from greek, a-tomos: un-divisible).

Mereology based on such items is called atomistic mereology.

However, in order not to confuse the lexicon between mereology and physics (in which an atom is a divisible physical entity) we prefer to call it &apos;elementary&apos;, recalling the concept of elementary particle coming from the standard particles model.</rdfs:comment>
        <rdfs:label xml:lang="en">elementary</rdfs:label>
    </owl:Class>
    


    <!-- http://emmc.info/emmo-core#EMMO_29072ec4_ffcb_42fb_bdc7_26f05a2e9873 -->

    <owl:Class rdf:about="http://emmc.info/emmo-core#EMMO_29072ec4_ffcb_42fb_bdc7_26f05a2e9873">
        <rdfs:subClassOf rdf:resource="http://emmc.info/emmo-core#EMMO_eb3a768e_d53e_4be9_a23b_0714833c36de"/>
        <rdfs:subClassOf>
            <owl:Restriction>
                <owl:onProperty rdf:resource="http://emmc.info/emmo-core#EMMO_17e27c22_37e1_468c_9dd7_95e137f73e7f"/>
                <owl:allValuesFrom rdf:resource="http://emmc.info/emmo-core#EMMO_29072ec4_ffcb_42fb_bdc7_26f05a2e9873"/>
            </owl:Restriction>
        </rdfs:subClassOf>
        <emmo-core:EMMO_70fe84ff_99b6_4206_a9fc_9a8931836d84>A &apos;item&apos; that has no &apos;physical&apos; parts.</emmo-core:EMMO_70fe84ff_99b6_4206_a9fc_9a8931836d84>
        <rdfs:label xml:lang="en">void</rdfs:label>
    </owl:Class>
    


    <!-- http://emmc.info/emmo-core#EMMO_2d2ecd97_067f_4d0e_950c_d746b7700a31 -->

    <owl:Class rdf:about="http://emmc.info/emmo-core#EMMO_2d2ecd97_067f_4d0e_950c_d746b7700a31">
        <rdfs:subClassOf rdf:resource="http://emmc.info/emmo-core#EMMO_802d3e92_8770_4f98_a289_ccaaab7fdddf"/>
        <rdfs:subClassOf>
            <owl:Restriction>
                <owl:onProperty rdf:resource="http://emmc.info/emmo-core#EMMO_6b7276a4_4b9d_440a_b577_0277539c0fc4"/>
                <owl:someValuesFrom rdf:resource="http://emmc.info/emmo-core#EMMO_eb3a768e_d53e_4be9_a23b_0714833c36de"/>
            </owl:Restriction>
        </rdfs:subClassOf>
        <emmo-core:EMMO_967080e5_2f42_4eb2_a3a9_c58143e835f9>The class of all individuals that stands for a real world not self-connected object.</emmo-core:EMMO_967080e5_2f42_4eb2_a3a9_c58143e835f9>
        <rdfs:comment>A &apos;collection&apos; individual is a sign that stands for a non-self-connected real world object.

A &apos;collection&apos; individual is related to each &apos;item&apos; individuals of the collection (i.e. the members) through the membership relation.

An &apos;item&apos; individual stands for a real world self-connected object which can be represented as a whole made of connected parts (e.g. a car made of components).</rdfs:comment>
        <rdfs:comment>Formally, &apos;collection&apos; is axiomatized as the class of individuals that &apos;has_member&apos; some &apos;item&apos;.

A &apos;collection&apos; cannot have as member another &apos;collection&apos;.</rdfs:comment>
        <rdfs:comment>e.g. the collection of users of a particular software, the collection of atoms that have been part of that just dissociated molecule, or even the collection of atoms that are part of a molecule considered as single individual non-connected objects and not as a mereotopological self-connected fusion.</rdfs:comment>
        <rdfs:label xml:lang="en">collection</rdfs:label>
    </owl:Class>
    


    <!-- http://emmc.info/emmo-core#EMMO_3f9ae00e_810c_4518_aec2_7200e424cf68 -->

    <owl:Class rdf:about="http://emmc.info/emmo-core#EMMO_3f9ae00e_810c_4518_aec2_7200e424cf68">
        <rdfs:subClassOf rdf:resource="http://emmc.info/emmo-core#EMMO_eb3a768e_d53e_4be9_a23b_0714833c36de"/>
        <rdfs:subClassOf>
            <owl:Restriction>
                <owl:onProperty rdf:resource="http://emmc.info/emmo-core#EMMO_9380ab64_0363_4804_b13f_3a8a94119a76"/>
                <owl:allValuesFrom rdf:resource="http://www.w3.org/2002/07/owl#Nothing"/>
            </owl:Restriction>
        </rdfs:subClassOf>
        <emmo-core:EMMO_967080e5_2f42_4eb2_a3a9_c58143e835f9>An &apos;emmo&apos; that can&apos;t be further divided in time nor in space.</emmo-core:EMMO_967080e5_2f42_4eb2_a3a9_c58143e835f9>
        <emmo-core:EMMO_b432d2d5_25f4_4165_99c5_5935a7763c1a>For a physics based ontology, like the EMMO, the &apos;quantum&apos; can stand for the smallest identifiable portion of spacetime defined by the Planck limit in length (1.616e-35 m) and time (5.39e-44 s).

For a manpower management ontology, a &apos;quantum&apos; can stand for an hour (time) of a worker (space) activity.</emmo-core:EMMO_b432d2d5_25f4_4165_99c5_5935a7763c1a>
        <rdfs:comment>A &apos;quantum&apos; is the most fundamental subclass of &apos;item&apos;, since we consider it as the smallest possible self-connected 4D real world object.

The quantum concept recalls the fact that there is lower epistemological limit to our knowledge of the universe, related to the uncertainity principle.</rdfs:comment>
        <rdfs:comment>A &apos;quantum&apos; stands for a 4D real world object.</rdfs:comment>
        <rdfs:comment>A quantum is the EMMO mereological a-tomic entity. 

To avoid confusion with the concept of atom coming from physics, we will use the expression quantum mereology, instead of a-tomistic mereology.</rdfs:comment>
        <rdfs:label xml:lang="en">quantum</rdfs:label>
    </owl:Class>
    


    <!-- http://emmc.info/emmo-core#EMMO_802d3e92_8770_4f98_a289_ccaaab7fdddf -->

    <owl:Class rdf:about="http://emmc.info/emmo-core#EMMO_802d3e92_8770_4f98_a289_ccaaab7fdddf">
        <owl:equivalentClass>
            <owl:Restriction>
                <owl:onProperty>
                    <rdf:Description>
                        <owl:inverseOf rdf:resource="http://emmc.info/emmo-core#EMMO_17e27c22_37e1_468c_9dd7_95e137f73e7f"/>
                    </rdf:Description>
                </owl:onProperty>
                <owl:hasValue rdf:resource="http://emmc.info/emmo-core#EMMO_08cb807c_e626_447b_863f_e2835540e918"/>
            </owl:Restriction>
        </owl:equivalentClass>
        <rdfs:subClassOf>
            <owl:Restriction>
                <owl:onProperty rdf:resource="http://emmc.info/emmo-core#EMMO_17e27c22_37e1_468c_9dd7_95e137f73e7f"/>
                <owl:someValuesFrom rdf:resource="http://emmc.info/emmo-core#EMMO_3f9ae00e_810c_4518_aec2_7200e424cf68"/>
            </owl:Restriction>
        </rdfs:subClassOf>
        <owl:disjointUnionOf rdf:parseType="Collection">
            <rdf:Description rdf:about="http://emmc.info/emmo-core#EMMO_2d2ecd97_067f_4d0e_950c_d746b7700a31"/>
            <rdf:Description rdf:about="http://emmc.info/emmo-core#EMMO_eb3a768e_d53e_4be9_a23b_0714833c36de"/>
        </owl:disjointUnionOf>
        <emmo-core:EMMO_967080e5_2f42_4eb2_a3a9_c58143e835f9>The class representing the collection of all the individuals declared in this ontology that stand for real world objects.</emmo-core:EMMO_967080e5_2f42_4eb2_a3a9_c58143e835f9>
        <rdfs:comment>&apos;emmo&apos; is the disjoint union of &apos;item&apos; and &apos;collection&apos; (covering axiom).

The union implies that &apos;emmo&apos; individuals can only be &apos;item&apos; individuals (standing for self-connected real world objects) or &apos;collection&apos; individuals (standing for a collection of disconnected items).

Disjointness means that a &apos;collection&apos; individual cannot be an &apos;item&apos; individual and viceversa, meaning that a real world object cannot be self-connected and non-self connected at the same time.</rdfs:comment>
        <rdfs:comment>For the EMMO the whole universe is represented at meta-ontological level (i.e. the representational level that includes the ontologist, the ontology and the universe) as a 4D path-connected topological manifold (i.e. the spacetime).

Mereotopology is the fundamental logical representation used to characterize the universe and to provide the definitions for the EMMO concepts at interpreter&apos;s level.

A real world object is then a 4D topological sub-region of the universe. 

A universe sub-region is isolated and defined as a real world object by the ontologist. Then, through a semiotic process that occurs at the meta-ontological level (i.e. outside the ontology). an ontology entity (e.g. an OWL individual) is assigned to represent that real object. 

The fundamental distinction between real world objects upon which the EMMO is based in self-connectedness: a real world object can be self-connected xor not self-connected.</rdfs:comment>
        <rdfs:comment>In the EMMO we will refer to the universe as a Minkowski space, restricting the ontology to special relativity only. However, exension to general relativity, will adding more complexity, should not change the overall approach.</rdfs:comment>
        <rdfs:comment>Parthood relations does not change dimensionality of an &apos;emmo&apos; individual, i.e. every part of a real world object always retains its 4D dimensionality. 

The smallest part is a &apos;quantum&apos;, that has no proper parts.

It follows that, for the EMMO, real world objects of dimensionality lower than 4D do not exist (e.g. surfaces, lines).</rdfs:comment>
        <rdfs:label xml:lang="en">emmo</rdfs:label>
    </owl:Class>
    


    <!-- http://emmc.info/emmo-core#EMMO_c5ddfdba_c074_4aa4_ad6b_1ac4942d300d -->

    <owl:Class rdf:about="http://emmc.info/emmo-core#EMMO_c5ddfdba_c074_4aa4_ad6b_1ac4942d300d">
        <rdfs:subClassOf rdf:resource="http://emmc.info/emmo-core#EMMO_eb3a768e_d53e_4be9_a23b_0714833c36de"/>
        <rdfs:subClassOf>
            <owl:Restriction>
                <owl:onProperty rdf:resource="http://emmc.info/emmo-core#EMMO_17e27c22_37e1_468c_9dd7_95e137f73e7f"/>
                <owl:someValuesFrom rdf:resource="http://emmc.info/emmo-core#EMMO_0f795e3e_c602_4577_9a43_d5a231aa1360"/>
            </owl:Restriction>
        </rdfs:subClassOf>
        <rdfs:subClassOf>
            <owl:Restriction>
                <owl:onProperty rdf:resource="http://emmc.info/emmo-core#EMMO_7afbed84_7593_4a23_bd88_9d9c6b04e8f6"/>
                <owl:allValuesFrom rdf:resource="http://emmc.info/emmo-core#EMMO_c5ddfdba_c074_4aa4_ad6b_1ac4942d300d"/>
            </owl:Restriction>
        </rdfs:subClassOf>
        <emmo-core:EMMO_967080e5_2f42_4eb2_a3a9_c58143e835f9>A &apos;item&apos; that is an &apos;elementary&apos; or has some &apos;elementary&apos; as proper parts and whose temporal proper parts are only &apos;physical&apos;-s (i.e. it can be perceived without interruptions in time).</emmo-core:EMMO_967080e5_2f42_4eb2_a3a9_c58143e835f9>
        <rdfs:comment>A &apos;physical&apos; is the class that contains all the individuals that stand for real world objects that interact physically with the interpreter.

Perception is a subcategory of interaction.

A physical must be perceived through physical interaction by the ontologist. Then the ontologist can declare an individual standing for the physical object just perceived.</rdfs:comment>
        <rdfs:comment>A &apos;physical&apos; must include at least an &apos;elementary&apos; part, but can also include void parts.

A &apos;physical&apos; may include as part also the &apos;void&apos; surrounding or enclosed by its &apos;physical&apos; sub parts.

There are no particular criteria for &apos;physical&apos;-s structure, except that is made of some &apos;elementary&apos;-s as proper parts and not only &apos;void&apos;.

This is done in order to:
a) take into account the quantum nature of physical systems, in which the actual position of sub-components (e.g. electrons in an atom) is not known except for its probability distribution function (according to the Copenhagen interpretation.)
b) take into account the fact that large entities (e.g. devices, cars, materials) have some void into them.

e.g. a &apos;spacetime&apos; that has spatial parts an atom and a cubic light year of &apos;void&apos; extending for some time can be a &apos;physical&apos; individual.</rdfs:comment>
        <rdfs:comment>A &apos;physical&apos; with dimensions other than 4D cannot exist, following the restriction of the parent &apos;emmo&apos; class.

It follows from the fact that perception is always a process (e.g. it unfolds in time).

e.g. you always have an aperture time when you take a picture or measure a property. Instantaneous perceptions are idealizations (abstractions) or a very small time measurement.</rdfs:comment>
        <rdfs:comment>In the EMMO there are no relations such as &apos;occupies_space&apos;, since &apos;physical&apos;-s are themselves the 4D region.</rdfs:comment>
        <rdfs:comment>The EMMO can be used to represent real world entities as &apos;physical&apos;-s that are easy to connect to classical or quantum mechanical based models.

Classical mechanics poses no representational issues, for the EMMO: the 4D representation of &apos;physical&apos;-s is consistent with classical physics systems.

However, the representation of &apos;physical&apos;-s that are typically analized through quantum mechanics (e.g. molecules, atoms, clusters), is not straightforward.

1) De Broglie - Bohm interpretation
The most simple approach is to rely on Bohmian mechanics, in which each particle is supposed to exists in a specific position between measurements (hidden variables approach), while its trajectory is calculated using a Guiding Equation based on a quantum field calculated with the Schroedinger Equation.

While this approach is really easy to implement in an ontology, since each entity has its own well defined 4D region, its mathematical representation failed to receive large consensus due to the difficulties to include relativistic effects, to be extended to subnuclear scale and the strong non-locality assumtpion of the quantum field.

Nevertheless, the Bohmian mechanics is a numerical approach that is used in electronic models to reduce the computational effort of the solution of Schroedinger Equation.

In practice, an EMMO user can declare a &apos;physical&apos; individual that stand for the whole quantum system to be described, and at the same time all sub-parts individuals can be declared, having them a well defined position in time, according to De Broglie - Bohm interpretation. The Hamiltonian can be calculated by considering the sub-part individuals.

&apos;physical&apos;-s are then made of &apos;physical&apos; parts and &apos;void&apos; parts that stand for the space between &apos;physical&apos;-s (e.g. the void between electrons and nucleus in an atom).

2) Copenhagen interpretation
In this interpretation the properties (e.g. energy level, position, spin) of a particle are not defined in the interval between two measurements and the quantum system is entangled (i.e. properties of particles in the sysyem are correlated) and described by a global wavefunction obtained solving the Schroedinger Equation. 

Upon measurement, the wavefunction collapses to a combination of close eigenstates that provide information about bservables of the system components (e.g. position, energy).

The EMMO can be used to represent &apos;physical&apos;-s that can be related to Copenhagen based models. In practice, the user should follow these steps:

a) define the quantum system as a &apos;physical&apos; individual (e.g. an H2 molecule) under a specific class (e.g. &apos;h2_molecule&apos;). This individual is the whole.

b) define the axioms of the  class that describe how many sub-parts are expected for the whole and their class types (e.g. &apos;h2_molecule&apos; has axioms &apos;has_proper_part exactly 2 electron&apos; and &apos;has_proper_part exactly 2 nucleus)

c) the user can now connect the whole to a Schroedinger equation based model whose Hamiltonian is calculated trough the information coming only from the axioms. No individuals are declared for the subparts!

d) a measurement done on the quantum system that provides information on the sub-part observables is interpreted as wavefunction collapse and leads to the end of the whole and the declaration of the sub-parts individuals which can be themselves other quantum systems 

e.g. if the outer electron of the H2 molecule interacts with another entity defining its state, then the whole that stands for the entangled H2 molecule becomes a &apos;physical&apos; made of an electron individual, a quantum system made of one electron and two nuclei and the void between them.

e.g. in the Born-Oppenheimer approximation the user represent the atom by un-entangling nucleus and electronic cloud. The un-entanglement comes in the form of declaration of individual as parts.

e.g. the double slit experiment can be represent in the EMMO as:
a) before the slit: a &apos;physical&apos; that extend in space and has parts &apos;electron&apos; and &apos;void&apos;, called &apos;single_electron_wave_function&apos;. &apos;electron&apos; and &apos;void&apos; are only in the axioms and not decalred individuals.
b) during slit passage: a &apos;physical&apos; made of one declared individual, the &apos;electron&apos;.
c) after the slit: again &apos;single_electron_wave_function&apos;
d) upon collision with the detector:  &apos;physical&apos; made of one declared individual, the &apos;electron&apos;.</rdfs:comment>
        <rdfs:comment>The purpose of the &apos;physical&apos; branch is to provide a representation of the real world objects, while the models used to explain or predict the behaviour of the real world objects lay under the &apos;semiotic&apos; branch.

More than one model can be connected to the same &apos;physical&apos;.

e.g. Navier-Stokes or Euler equation applied to the same fluid</rdfs:comment>
        <rdfs:label xml:lang="en">physical</rdfs:label>
    </owl:Class>
    


    <!-- http://emmc.info/emmo-core#EMMO_eb3a768e_d53e_4be9_a23b_0714833c36de -->

    <owl:Class rdf:about="http://emmc.info/emmo-core#EMMO_eb3a768e_d53e_4be9_a23b_0714833c36de">
        <rdfs:subClassOf rdf:resource="http://emmc.info/emmo-core#EMMO_802d3e92_8770_4f98_a289_ccaaab7fdddf"/>
        <owl:disjointUnionOf rdf:parseType="Collection">
            <rdf:Description rdf:about="http://emmc.info/emmo-core#EMMO_29072ec4_ffcb_42fb_bdc7_26f05a2e9873"/>
            <rdf:Description rdf:about="http://emmc.info/emmo-core#EMMO_c5ddfdba_c074_4aa4_ad6b_1ac4942d300d"/>
        </owl:disjointUnionOf>
        <emmo-core:EMMO_967080e5_2f42_4eb2_a3a9_c58143e835f9>The class of individuals that stand for single real world self-connected objects.</emmo-core:EMMO_967080e5_2f42_4eb2_a3a9_c58143e835f9>
        <rdfs:comment>A real world object is self-connected if any two parts that make up the whole are connected to each other (here the concept of connection is primitive). 

Alternatively, using the primitive path-connectivity concept we can define a self-connected real world object as an object for which each couple of points is path-connected.</rdfs:comment>
        <rdfs:comment>An &apos;item&apos; individual stands for a real world self-connected object which can be represented as a whole made of connected parts (e.g. a car made of components).

In the EMMO, connectivity is the topological foundation of causality.

All physical systems, i.e. systems whose behaviour is explained by physics laws, are always represented by &apos;item&apos;-s.

Members of a &apos;collection&apos; lack of causality connection, i.e. they do not constitute a physical system as a whole.</rdfs:comment>
        <rdfs:label xml:lang="en">item</rdfs:label>
    </owl:Class>
    


    <!-- http://emmc.info/emmo-granularity#EMMO_36c79456_e29c_400d_8bd3_0eedddb82652 -->

    <owl:Class rdf:about="http://emmc.info/emmo-granularity#EMMO_36c79456_e29c_400d_8bd3_0eedddb82652">
        <rdfs:subClassOf rdf:resource="http://emmc.info/emmo-granularity#EMMO_52211e5e_d767_4812_845e_eb6b402c476a"/>
        <rdfs:subClassOf>
            <owl:Class>
                <owl:unionOf rdf:parseType="Collection">
                    <rdf:Description rdf:about="http://emmc.info/emmo-core#EMMO_0f795e3e_c602_4577_9a43_d5a231aa1360"/>
                    <owl:Restriction>
                        <owl:onProperty rdf:resource="http://emmc.info/emmo-granularity#EMMO_b2282816_b7a3_44c6_b2cb_3feff1ceb7fe"/>
                        <owl:someValuesFrom rdf:resource="http://emmc.info/emmo-granularity#EMMO_52211e5e_d767_4812_845e_eb6b402c476a"/>
                    </owl:Restriction>
                </owl:unionOf>
            </owl:Class>
        </rdfs:subClassOf>
        <emmo-core:EMMO_967080e5_2f42_4eb2_a3a9_c58143e835f9>An &apos;existent&apos; whose spatial direct parts extends from one change in spatial direct part cardinality (i.e. the number of spatial direct parts) to the immidiate next change.</emmo-core:EMMO_967080e5_2f42_4eb2_a3a9_c58143e835f9>
        <emmo-core:EMMO_b432d2d5_25f4_4165_99c5_5935a7763c1a>e.g. the existent in my glass is declared at t = t_start as made of two direct parts: the ice and the water. It will continue to exists as state as long as the ice is completely melt at t = t_end. The new state will be completely made of water. Between t_start and t_end there is an exchange of molecules between the ice and the water, but this does not affect the existence of the two states.

If we partition the existent in my glass as ice surrounded by several molecules (we do not use the object water as direct part) then the appearance of a molecule coming from the ice will cause a state to end and another state to begin.</emmo-core:EMMO_b432d2d5_25f4_4165_99c5_5935a7763c1a>
        <rdfs:comment>Direct partitions declaration is a choice of the ontology developer that choses the classes to be used as direct parts, according to its own world view.

A &apos;state&apos; can always be direct partitioned in &apos;elementary&apos;-s and &apos;void&apos; or &apos;physical&apos;.

e.g. the water in my glass can be seen as a single object without declaring direct parts, or as made of H2O molecules direct parts.</rdfs:comment>
        <rdfs:comment>The definition of &apos;state&apos; implies that its spatial direct parts (i.e. &apos;physicals&apos;) are not gained or lost during its temporal extension (they exist from the left to the right side of the time interval), so that the granularity of a &apos;state&apos; is constant.

This does not mean that there cannot be a change in the internal structure of the &apos;state&apos; direct parts. It means only that this change must not affect the existence of the direct part itself.

There is no change in granularity or cardinality of direct parts within a &apos;state&apos;.

Also, the &apos;state&apos; must cover all the time interval between two successive cardinality changes.

The use of spatial direct parthood in &apos;state&apos; definition means that a &apos;state&apos; cannot overlap in space another &apos;state&apos;.</rdfs:comment>
        <rdfs:comment>The usefulness of &apos;state&apos; is that it makes it possible to describe the evolution in time of an &apos;existent&apos; in terms of series of &apos;state&apos;-s that can take into account the disappearance or appearance of parts within a &apos;physical&apos;. 

A &apos;state&apos; is a recognizable granularity level of matter, in the sense that its direct parts do not appear or disappear within its lifetime as it can be for a generic &apos;existent&apos;.</rdfs:comment>
        <rdfs:comment>There is no change in granularity or cardinality of parts within a state.

The use of spatial direct parthood in state definition means that a state cannot overlap in space another state that is direct part of the same whole.</rdfs:comment>
        <rdfs:label xml:lang="en">state</rdfs:label>
    </owl:Class>
    


    <!-- http://emmc.info/emmo-granularity#EMMO_52211e5e_d767_4812_845e_eb6b402c476a -->

    <owl:Class rdf:about="http://emmc.info/emmo-granularity#EMMO_52211e5e_d767_4812_845e_eb6b402c476a">
        <rdfs:subClassOf rdf:resource="http://emmc.info/emmo-core#EMMO_c5ddfdba_c074_4aa4_ad6b_1ac4942d300d"/>
        <rdfs:subClassOf>
            <owl:Class>
                <owl:unionOf rdf:parseType="Collection">
                    <rdf:Description rdf:about="http://emmc.info/emmo-granularity#EMMO_36c79456_e29c_400d_8bd3_0eedddb82652"/>
                    <owl:Restriction>
                        <owl:onProperty rdf:resource="http://emmc.info/emmo-granularity#EMMO_65a2c5b8_e4d8_4a51_b2f8_e55effc0547d"/>
                        <owl:someValuesFrom rdf:resource="http://emmc.info/emmo-granularity#EMMO_36c79456_e29c_400d_8bd3_0eedddb82652"/>
                    </owl:Restriction>
                </owl:unionOf>
            </owl:Class>
        </rdfs:subClassOf>
        <emmo-core:EMMO_70fe84ff_99b6_4206_a9fc_9a8931836d84>A &apos;item&apos; which is a &apos;state&apos; or made only of &apos;state&apos; temporal direct parts.</emmo-core:EMMO_70fe84ff_99b6_4206_a9fc_9a8931836d84>
        <rdfs:comment>&apos;existent&apos; is the most important class to be used for representing real world physical objects under a reductionistic (i.e. objects come from the composition of sub-part objects) and epistemological pluralistic (i.e. objects definitions are interpreter dependent) perspectives . 

&apos;existent&apos; class collects all individuals that stand for real world physical objects that can be structured in well defined temporal sub-parts called states through the temporal direct parthood.

This class provides a granularity hierarchy in time, that provides a way to axiomatize tessellation principles for a specific whole with a non-transitivity relation that helps to retain the granularity levels.

e.g. a car, a supersaturated gas with nucleating nanoparticles, an atom that becomes ionized and then recombines with an electron.</rdfs:comment>
        <rdfs:comment>ex-sistere (latin): to stay (to persist through time) outside others of the same type (to be distinct from the rest).</rdfs:comment>
        <rdfs:label xml:lang="en">existent</rdfs:label>
    </owl:Class>
    


    <!-- http://emmc.info/emmo-process#EMMO_43e9a05d_98af_41b4_92f6_00f79a09bfce -->

    <owl:Class rdf:about="http://emmc.info/emmo-process#EMMO_43e9a05d_98af_41b4_92f6_00f79a09bfce">
        <rdfs:subClassOf rdf:resource="http://emmc.info/emmo-core#EMMO_c5ddfdba_c074_4aa4_ad6b_1ac4942d300d"/>
        <rdfs:subClassOf>
            <owl:Restriction>
                <owl:onProperty rdf:resource="http://emmc.info/emmo-process#EMMO_ae2d1a96_bfa1_409a_a7d2_03d69e8a125a"/>
                <owl:someValuesFrom rdf:resource="http://emmc.info/emmo-process#EMMO_49804605_c0fe_4538_abda_f70ba1dc8a5d"/>
            </owl:Restriction>
        </rdfs:subClassOf>
        <emmo-core:EMMO_70fe84ff_99b6_4206_a9fc_9a8931836d84>A &apos;process&apos; is defined as a temporal part of a &apos;physical&apos; that is categorized in a primitive process subclass according to what type of process we want to represent.

Following the common definition of process, every &apos;physical&apos; is a process since every 4D object always has a time dimension. However, in the EMMO we restrict the meaning of the word process to &apos;physical&apos;-s whose evolution in time have a particular meaning for the ontologist. 

i.e. a &apos;process&apos; is not only something that unfolds in time (which is automatically represented in a 4D ontology), but something happening that has a meaning for the interpreter.</emmo-core:EMMO_70fe84ff_99b6_4206_a9fc_9a8931836d84>
        <emmo-core:EMMO_967080e5_2f42_4eb2_a3a9_c58143e835f9>A &apos;process&apos; is always a &apos;physical&apos;, since a &apos;void&apos; does not have elements that evolves in time.</emmo-core:EMMO_967080e5_2f42_4eb2_a3a9_c58143e835f9>
        <emmo-core:EMMO_967080e5_2f42_4eb2_a3a9_c58143e835f9>A temporal part of a &apos;physical&apos; that identifies a particular type of evolution in time.</emmo-core:EMMO_967080e5_2f42_4eb2_a3a9_c58143e835f9>
        <rdfs:label xml:lang="en">process</rdfs:label>
    </owl:Class>
    


    <!-- http://emmc.info/emmo-process#EMMO_49804605_c0fe_4538_abda_f70ba1dc8a5d -->

    <owl:Class rdf:about="http://emmc.info/emmo-process#EMMO_49804605_c0fe_4538_abda_f70ba1dc8a5d">
        <rdfs:subClassOf rdf:resource="http://emmc.info/emmo-core#EMMO_c5ddfdba_c074_4aa4_ad6b_1ac4942d300d"/>
        <emmo-core:EMMO_967080e5_2f42_4eb2_a3a9_c58143e835f9>A portion of a &apos;process&apos; that participates to the &apos;process&apos; with a specific role.</emmo-core:EMMO_967080e5_2f42_4eb2_a3a9_c58143e835f9>
        <rdfs:comment>In the EMMO the relation of participation to a process falls under mereotopology.</rdfs:comment>
        <rdfs:label xml:lang="en">participant</rdfs:label>
    </owl:Class>
    


    <!-- http://emmc.info/emmo-properties#EMMO_10a5fd39_06aa_4648_9e70_f962a9cb2069 -->

    <owl:Class rdf:about="http://emmc.info/emmo-properties#EMMO_10a5fd39_06aa_4648_9e70_f962a9cb2069">
        <rdfs:subClassOf rdf:resource="http://emmc.info/emmo-semiotics#EMMO_008fd3b2_4013_451f_8827_52bceab11841"/>
        <rdfs:subClassOf>
            <owl:Restriction>
                <owl:onProperty rdf:resource="http://emmc.info/emmo-process#EMMO_ae2d1a96_bfa1_409a_a7d2_03d69e8a125a"/>
                <owl:someValuesFrom rdf:resource="http://emmc.info/emmo-properties#EMMO_1b52ee70_121e_4d8d_8419_3f97cd0bd89c"/>
            </owl:Restriction>
        </rdfs:subClassOf>
        <rdfs:subClassOf>
            <owl:Restriction>
                <owl:onProperty rdf:resource="http://emmc.info/emmo-process#EMMO_ae2d1a96_bfa1_409a_a7d2_03d69e8a125a"/>
                <owl:someValuesFrom rdf:resource="http://emmc.info/emmo-properties#EMMO_b7bcff25_ffc3_474e_9ab5_01b1664bd4ba"/>
            </owl:Restriction>
        </rdfs:subClassOf>
        <emmo-core:EMMO_967080e5_2f42_4eb2_a3a9_c58143e835f9>A &apos;semiosis&apos; that involves an &apos;observer&apos; that perceives another &apos;entity&apos; (the &apos;object&apos;) through a specific perception mechanism and produces a &apos;property&apos; (the &apos;sign&apos;) that stands for the result of that particular perception.</emmo-core:EMMO_967080e5_2f42_4eb2_a3a9_c58143e835f9>
        <rdfs:label xml:lang="en">observation</rdfs:label>
    </owl:Class>
    


    <!-- http://emmc.info/emmo-properties#EMMO_1b52ee70_121e_4d8d_8419_3f97cd0bd89c -->

    <owl:Class rdf:about="http://emmc.info/emmo-properties#EMMO_1b52ee70_121e_4d8d_8419_3f97cd0bd89c">
        <rdfs:subClassOf rdf:resource="http://emmc.info/emmo-semiotics#EMMO_0527413c_b286_4e9c_b2d0_03fb2a038dee"/>
        <rdfs:subClassOf>
            <owl:Restriction>
                <owl:onProperty>
                    <rdf:Description>
                        <owl:inverseOf rdf:resource="http://emmc.info/emmo-process#EMMO_ae2d1a96_bfa1_409a_a7d2_03d69e8a125a"/>
                    </rdf:Description>
                </owl:onProperty>
                <owl:someValuesFrom rdf:resource="http://emmc.info/emmo-properties#EMMO_10a5fd39_06aa_4648_9e70_f962a9cb2069"/>
            </owl:Restriction>
        </rdfs:subClassOf>
        <emmo-core:EMMO_967080e5_2f42_4eb2_a3a9_c58143e835f9>An &apos;interpreter&apos; that perceives another &apos;entity&apos; (the &apos;object&apos;) through a specific perception mechanism and produces a &apos;property&apos; (the &apos;sign&apos;) that stands for the result of that particular perception.</emmo-core:EMMO_967080e5_2f42_4eb2_a3a9_c58143e835f9>
        <rdfs:label xml:lang="en">observer</rdfs:label>
    </owl:Class>
    


    <!-- http://emmc.info/emmo-properties#EMMO_251cfb4f_5c75_4778_91ed_6c8395212fd8 -->

    <owl:Class rdf:about="http://emmc.info/emmo-properties#EMMO_251cfb4f_5c75_4778_91ed_6c8395212fd8">
        <rdfs:subClassOf rdf:resource="http://emmc.info/emmo-properties#EMMO_b7bcff25_ffc3_474e_9ab5_01b1664bd4ba"/>
        <emmo-core:EMMO_967080e5_2f42_4eb2_a3a9_c58143e835f9>A &apos;property&apos; that cannot be univocally determined and depends on an agent (e.g. a human individual, a community) acting as black-box.</emmo-core:EMMO_967080e5_2f42_4eb2_a3a9_c58143e835f9>
        <emmo-core:EMMO_b432d2d5_25f4_4165_99c5_5935a7763c1a>The beauty of that girl.
The style of your clothing.</emmo-core:EMMO_b432d2d5_25f4_4165_99c5_5935a7763c1a>
        <rdfs:comment>The word subjective means that a non-well defined or an unknown procedure is used for the definition of the property.

This happens due to e.g. the complexity of the object, the lack of a underlying model for the representation of the object, the non-well specified meaning of the property symbols. 

A &apos;subjective_property&apos; cannot be used to univocally compare &apos;object&apos;-s.

e.g. you cannot evaluate the beauty of a person on objective basis.</rdfs:comment>
        <rdfs:label xml:lang="en">subjective property</rdfs:label>
    </owl:Class>
    


    <!-- http://emmc.info/emmo-properties#EMMO_2a888cdf_ec4a_4ec5_af1c_0343372fc978 -->

    <owl:Class rdf:about="http://emmc.info/emmo-properties#EMMO_2a888cdf_ec4a_4ec5_af1c_0343372fc978">
        <rdfs:subClassOf rdf:resource="http://emmc.info/emmo-properties#EMMO_b7bcff25_ffc3_474e_9ab5_01b1664bd4ba"/>
        <emmo-core:EMMO_967080e5_2f42_4eb2_a3a9_c58143e835f9>A &apos;property&apos; that is determined by each &apos;observer&apos; following a well defined &apos;observation&apos; procedure through a specific perception channel.</emmo-core:EMMO_967080e5_2f42_4eb2_a3a9_c58143e835f9>
        <rdfs:comment>The word objective does not mean that each observation will provide the same results. It means that the observation followed a well defined procedure.</rdfs:comment>
        <rdfs:label xml:lang="en">objective property</rdfs:label>
    </owl:Class>
    


    <!-- http://emmc.info/emmo-properties#EMMO_b7bcff25_ffc3_474e_9ab5_01b1664bd4ba -->

    <owl:Class rdf:about="http://emmc.info/emmo-properties#EMMO_b7bcff25_ffc3_474e_9ab5_01b1664bd4ba">
        <rdfs:subClassOf rdf:resource="http://emmc.info/emmo-semiotics#EMMO_057e7d57_aff0_49de_911a_8861d85cef40"/>
        <rdfs:subClassOf rdf:resource="http://emmc.info/emmo-semiotics#EMMO_35d2e130_6e01_41ed_94f7_00b333d46cf9"/>
        <rdfs:subClassOf>
            <owl:Restriction>
                <owl:onProperty>
                    <rdf:Description>
                        <owl:inverseOf rdf:resource="http://emmc.info/emmo-properties#EMMO_e1097637_70d2_4895_973f_2396f04fa204"/>
                    </rdf:Description>
                </owl:onProperty>
                <owl:someValuesFrom rdf:resource="http://emmc.info/emmo-core#EMMO_802d3e92_8770_4f98_a289_ccaaab7fdddf"/>
            </owl:Restriction>
        </rdfs:subClassOf>
        <owl:disjointUnionOf rdf:parseType="Collection">
            <rdf:Description rdf:about="http://emmc.info/emmo-properties#EMMO_251cfb4f_5c75_4778_91ed_6c8395212fd8"/>
            <rdf:Description rdf:about="http://emmc.info/emmo-properties#EMMO_2a888cdf_ec4a_4ec5_af1c_0343372fc978"/>
        </owl:disjointUnionOf>
        <emmo-core:EMMO_967080e5_2f42_4eb2_a3a9_c58143e835f9>A &apos;sign&apos; that stands for an &apos;object&apos; that the &apos;interpreter&apos; perceived through a well defined &apos;observation&apos; process.

(a property is always a partial representation of an &apos;object&apos; since it reflects the &apos;object&apos; capability to be part of a specific &apos;observation&apos; process)</emmo-core:EMMO_967080e5_2f42_4eb2_a3a9_c58143e835f9>
        <emmo-core:EMMO_b432d2d5_25f4_4165_99c5_5935a7763c1a>Hardness is a subclass of properties.

Vickers hardness is a subclass of hardness that involves the procedures and instruments defined by the standard hardness test.</emmo-core:EMMO_b432d2d5_25f4_4165_99c5_5935a7763c1a>
        <emmo-core:EMMO_b432d2d5_25f4_4165_99c5_5935a7763c1a>Let&apos;s define the class &apos;colour&apos; as the subclass of the properties that involve photon emission and an electromagnetic radiation sensible observer.

An individual C of this class &apos;colour&apos; can be defined be declaring the process individual (e.g. daylight illumination) and the observer (e.g. my eyes)

Stating that an entity E has_property C, we mean that it can be observed by such setup of process + observer (i.e. observed by my eyes under daylight).

This definition can be generalized by using a generic human eye, so that the observer can be a generic human.

This can be used in material characterization, to define exactly the type of measurement done, including the instrument type.</emmo-core:EMMO_b432d2d5_25f4_4165_99c5_5935a7763c1a>
        <rdfs:comment>We know real world entities through observation/perception.

A non-perceivable real world entity does not exist (or it exists on a plane of existance that has no intersection with us and we can say nothing about it).

Perception/observation of a real wolrd entity occurs when the entity stimulate an observer in a peculiar way through a well defined perception channel.

For this reason each property is related to a specific observation process which involves a specific observer with its own perception mechanisms.

The observation process (e.g. a look, a photo shot, a measurement) is performed  by an observer (e.g. you, a camera, an instrument) through a specific perception mechanism (e.g. retina impression, CMOS excitation, piezoelectric sensor activation) and involves an observed entity.

An observation is a semiotic process, since it stimulate an interpretant within the interpreter who can communicate the perception result to other interpreters through a sign which is the property. 

Property subclasses are specializations that depend on the type of observation processes.

e.g. the property &apos;colour&apos; is related to a process that involves emission or interaction of photon and an observer who can perceive electromagnetic radiation in the visible frequency range. 

Properties usually relies on symbolic systems (e.g. for colour it can be palette or RGB).</rdfs:comment>
        <rdfs:label xml:lang="en">property</rdfs:label>
    </owl:Class>
    


    <!-- http://emmc.info/emmo-semiotics#EMMO_008fd3b2_4013_451f_8827_52bceab11841 -->

    <owl:Class rdf:about="http://emmc.info/emmo-semiotics#EMMO_008fd3b2_4013_451f_8827_52bceab11841">
        <rdfs:subClassOf rdf:resource="http://emmc.info/emmo-process#EMMO_43e9a05d_98af_41b4_92f6_00f79a09bfce"/>
        <rdfs:subClassOf>
            <owl:Restriction>
                <owl:onProperty rdf:resource="http://emmc.info/emmo-process#EMMO_ae2d1a96_bfa1_409a_a7d2_03d69e8a125a"/>
                <owl:someValuesFrom rdf:resource="http://emmc.info/emmo-semiotics#EMMO_0527413c_b286_4e9c_b2d0_03fb2a038dee"/>
            </owl:Restriction>
        </rdfs:subClassOf>
        <rdfs:subClassOf>
            <owl:Restriction>
                <owl:onProperty rdf:resource="http://emmc.info/emmo-process#EMMO_c5aae418_1622_4d02_93c5_21159e28e6c1"/>
                <owl:someValuesFrom rdf:resource="http://emmc.info/emmo-semiotics#EMMO_6f5af708_f825_4feb_a0d1_a8d813d3022b"/>
            </owl:Restriction>
        </rdfs:subClassOf>
        <rdfs:subClassOf>
            <owl:Restriction>
                <owl:onProperty rdf:resource="http://emmc.info/emmo-process#EMMO_c5aae418_1622_4d02_93c5_21159e28e6c1"/>
                <owl:someValuesFrom rdf:resource="http://emmc.info/emmo-semiotics#EMMO_b21a56ed_f969_4612_a6ec_cb7766f7f31d"/>
            </owl:Restriction>
        </rdfs:subClassOf>
        <emmo-core:EMMO_967080e5_2f42_4eb2_a3a9_c58143e835f9>A &apos;process&apos;, that has participant an &apos;interpreter&apos;, that is aimed to produce a &apos;sign&apos; representing another participant, the &apos;interpreted&apos;.</emmo-core:EMMO_967080e5_2f42_4eb2_a3a9_c58143e835f9>
        <emmo-core:EMMO_b432d2d5_25f4_4165_99c5_5935a7763c1a>Me looking a cat and saying loud: &quot;Cat!&quot; -&gt; the semiosis process

me -&gt; interpreter
cat -&gt; object (in Peirce semiotics)
the cat perceived by my mind -&gt; interpretant
&quot;Cat!&quot; -&gt; sign, the produced sign</emmo-core:EMMO_b432d2d5_25f4_4165_99c5_5935a7763c1a>
        <rdfs:label xml:lang="en">semiosis</rdfs:label>
    </owl:Class>
    


    <!-- http://emmc.info/emmo-semiotics#EMMO_0527413c_b286_4e9c_b2d0_03fb2a038dee -->

    <owl:Class rdf:about="http://emmc.info/emmo-semiotics#EMMO_0527413c_b286_4e9c_b2d0_03fb2a038dee">
        <rdfs:subClassOf rdf:resource="http://emmc.info/emmo-semiotics#EMMO_b803f122_4acb_4064_9d71_c1e5fd091fc9"/>
        <rdfs:subClassOf>
            <owl:Restriction>
                <owl:onProperty rdf:resource="http://emmc.info/emmo-4d#EMMO_f68030be_94b8_4c61_a161_886468558054"/>
                <owl:someValuesFrom rdf:resource="http://emmc.info/emmo-semiotics#EMMO_054af807_85cd_4a13_8eba_119dfdaaf38b"/>
            </owl:Restriction>
        </rdfs:subClassOf>
        <emmo-core:EMMO_967080e5_2f42_4eb2_a3a9_c58143e835f9>The entity (or agent, or observer, or cognitive entity) who connects &apos;sign&apos;, &apos;interpretant&apos; and &apos;object&apos;.</emmo-core:EMMO_967080e5_2f42_4eb2_a3a9_c58143e835f9>
        <rdfs:label xml:lang="en">interpreter</rdfs:label>
    </owl:Class>
    


    <!-- http://emmc.info/emmo-semiotics#EMMO_054af807_85cd_4a13_8eba_119dfdaaf38b -->

    <owl:Class rdf:about="http://emmc.info/emmo-semiotics#EMMO_054af807_85cd_4a13_8eba_119dfdaaf38b">
        <rdfs:subClassOf rdf:resource="http://emmc.info/emmo-semiotics#EMMO_b21a56ed_f969_4612_a6ec_cb7766f7f31d"/>
        <rdfs:label xml:lang="en">interpretant</rdfs:label>
    </owl:Class>
    


    <!-- http://emmc.info/emmo-semiotics#EMMO_057e7d57_aff0_49de_911a_8861d85cef40 -->

    <owl:Class rdf:about="http://emmc.info/emmo-semiotics#EMMO_057e7d57_aff0_49de_911a_8861d85cef40">
        <rdfs:subClassOf rdf:resource="http://emmc.info/emmo-semiotics#EMMO_c74da218_9147_4f03_92d1_8894abca55f3"/>
        <rdfs:subClassOf>
            <owl:Class>
                <owl:unionOf rdf:parseType="Collection">
                    <rdf:Description rdf:about="http://emmc.info/emmo-semiotics#EMMO_a1083d0a_c1fb_471f_8e20_a98f881ad527"/>
                    <owl:Restriction>
                        <owl:onProperty rdf:resource="http://emmc.info/emmo-4d#EMMO_f68030be_94b8_4c61_a161_886468558054"/>
                        <owl:someValuesFrom rdf:resource="http://emmc.info/emmo-semiotics#EMMO_a1083d0a_c1fb_471f_8e20_a98f881ad527"/>
                    </owl:Restriction>
                </owl:unionOf>
            </owl:Class>
        </rdfs:subClassOf>
        <emmo-core:EMMO_70fe84ff_99b6_4206_a9fc_9a8931836d84>A &apos;symbol&apos; or a composition of &apos;symbol&apos;-s not necesarily respecting syntactic rules.</emmo-core:EMMO_70fe84ff_99b6_4206_a9fc_9a8931836d84>
        <emmo-core:EMMO_967080e5_2f42_4eb2_a3a9_c58143e835f9>An &apos;physical&apos; that stands for a symbolic object, i.e. a string of symbols from a specific alphabet.</emmo-core:EMMO_967080e5_2f42_4eb2_a3a9_c58143e835f9>
        <emmo-core:EMMO_b432d2d5_25f4_4165_99c5_5935a7763c1a>fe@è0
emmo
!5*a
cat</emmo-core:EMMO_b432d2d5_25f4_4165_99c5_5935a7763c1a>
        <rdfs:comment>In formal languages it is called a string of symbols.</rdfs:comment>
        <rdfs:label xml:lang="en">symbolic</rdfs:label>
    </owl:Class>
    


    <!-- http://emmc.info/emmo-semiotics#EMMO_0cd58641_824c_4851_907f_f4c3be76630c -->

    <owl:Class rdf:about="http://emmc.info/emmo-semiotics#EMMO_0cd58641_824c_4851_907f_f4c3be76630c">
        <rdfs:subClassOf rdf:resource="http://emmc.info/emmo-semiotics#EMMO_b21a56ed_f969_4612_a6ec_cb7766f7f31d"/>
        <emmo-core:EMMO_967080e5_2f42_4eb2_a3a9_c58143e835f9>A &apos;sign&apos; that stands for an &apos;objectì due to causal continguity.</emmo-core:EMMO_967080e5_2f42_4eb2_a3a9_c58143e835f9>
        <emmo-core:EMMO_b432d2d5_25f4_4165_99c5_5935a7763c1a>Smoke stands for a combustion process (a fire).

My facial expression stands for my emotional status.</emmo-core:EMMO_b432d2d5_25f4_4165_99c5_5935a7763c1a>
        <rdfs:label xml:lang="en">index</rdfs:label>
    </owl:Class>
    


    <!-- http://emmc.info/emmo-semiotics#EMMO_35d2e130_6e01_41ed_94f7_00b333d46cf9 -->

    <owl:Class rdf:about="http://emmc.info/emmo-semiotics#EMMO_35d2e130_6e01_41ed_94f7_00b333d46cf9">
        <rdfs:subClassOf rdf:resource="http://emmc.info/emmo-semiotics#EMMO_b21a56ed_f969_4612_a6ec_cb7766f7f31d"/>
        <emmo-core:EMMO_967080e5_2f42_4eb2_a3a9_c58143e835f9>A &apos;sign&apos; that stand for an &apos;object&apos; through convention, norm or habit, without any resemblance to it.</emmo-core:EMMO_967080e5_2f42_4eb2_a3a9_c58143e835f9>
        <rdfs:label xml:lang="en">conventional</rdfs:label>
    </owl:Class>
    


    <!-- http://emmc.info/emmo-semiotics#EMMO_50ea1ec5_f157_41b0_b46b_a9032f17ca10 -->

    <owl:Class rdf:about="http://emmc.info/emmo-semiotics#EMMO_50ea1ec5_f157_41b0_b46b_a9032f17ca10">
        <rdfs:subClassOf rdf:resource="http://emmc.info/emmo-semiotics#EMMO_057e7d57_aff0_49de_911a_8861d85cef40"/>
        <rdfs:subClassOf>
            <owl:Restriction>
                <owl:onProperty rdf:resource="http://emmc.info/emmo-core#EMMO_9380ab64_0363_4804_b13f_3a8a94119a76"/>
                <owl:someValuesFrom rdf:resource="http://emmc.info/emmo-semiotics#EMMO_a1083d0a_c1fb_471f_8e20_a98f881ad527"/>
            </owl:Restriction>
        </rdfs:subClassOf>
        <emmo-core:EMMO_967080e5_2f42_4eb2_a3a9_c58143e835f9>A composition of more than one &apos;symbol&apos;-s respecting a specific language syntactic rules (well-formed formula).</emmo-core:EMMO_967080e5_2f42_4eb2_a3a9_c58143e835f9>
        <emmo-core:EMMO_b432d2d5_25f4_4165_99c5_5935a7763c1a>The word &quot;cat&quot; considered as a collection of &apos;symbol&apos;-s respecting the rules of english language. 

In this example the &apos;symbolic&apos; entity &quot;cat&quot; is not related to the real cat, but it is only a word (like it would be to an italian person that ignores the meaning of this english word).

If an &apos;interpreter&apos; skilled in english language is involved in a &apos;semiotic&apos; process with this word, that &quot;cat&quot; became also a &apos;sign&apos; i.e. it became for the &apos;interpreter&apos; a representation for a real cat.</emmo-core:EMMO_b432d2d5_25f4_4165_99c5_5935a7763c1a>
        <rdfs:comment>In formal languages the terms word or well-formed formula are used with the same meaning.</rdfs:comment>
        <rdfs:label xml:lang="en">formula</rdfs:label>
    </owl:Class>
    


    <!-- http://emmc.info/emmo-semiotics#EMMO_6f5af708_f825_4feb_a0d1_a8d813d3022b -->

    <owl:Class rdf:about="http://emmc.info/emmo-semiotics#EMMO_6f5af708_f825_4feb_a0d1_a8d813d3022b">
        <owl:equivalentClass>
            <owl:Restriction>
                <owl:onProperty rdf:resource="http://emmc.info/emmo-semiotics#EMMO_60577dea_9019_4537_ac41_80b0fb563d41"/>
                <owl:someValuesFrom rdf:resource="http://emmc.info/emmo-semiotics#EMMO_b21a56ed_f969_4612_a6ec_cb7766f7f31d"/>
            </owl:Restriction>
        </owl:equivalentClass>
        <rdfs:subClassOf rdf:resource="http://emmc.info/emmo-semiotics#EMMO_b803f122_4acb_4064_9d71_c1e5fd091fc9"/>
        <emmo-core:EMMO_967080e5_2f42_4eb2_a3a9_c58143e835f9>The object, in Peirce semiotics.</emmo-core:EMMO_967080e5_2f42_4eb2_a3a9_c58143e835f9>
        <rdfs:comment>Here is assumed that the concept of &apos;object&apos; is always relative to a &apos;semiotic&apos; process. An &apos;object&apos; does not exists per se, but it&apos;s always part of an interpretation.

The EMMO relies on strong reductionism, i.e. everything real is a formless collection of elementary particles: we give a meaning to real world entities only by giving them boundaries and defining them using &apos;sign&apos;-s. 

In this way the &apos;sign&apos;-ed entity become and &apos;object&apos;, and the &apos;object&apos; is the basic entity needed in order to apply a logical formalism to the real world entities (i.e. we can speak of it through its sign, and use logics on it through its sign).</rdfs:comment>
        <rdfs:label xml:lang="en">object</rdfs:label>
    </owl:Class>
    


    <!-- http://emmc.info/emmo-semiotics#EMMO_a1083d0a_c1fb_471f_8e20_a98f881ad527 -->

    <owl:Class rdf:about="http://emmc.info/emmo-semiotics#EMMO_a1083d0a_c1fb_471f_8e20_a98f881ad527">
        <rdfs:subClassOf rdf:resource="http://emmc.info/emmo-semiotics#EMMO_057e7d57_aff0_49de_911a_8861d85cef40"/>
        <emmo-core:EMMO_967080e5_2f42_4eb2_a3a9_c58143e835f9>The class of individuals that stand for an elementary mark of a specific symbolic code (alphabet).</emmo-core:EMMO_967080e5_2f42_4eb2_a3a9_c58143e835f9>
        <emmo-core:EMMO_b432d2d5_25f4_4165_99c5_5935a7763c1a>The class of letter &quot;A&quot; is the symbol as idea and the letter A that you see on the screen is the mark.</emmo-core:EMMO_b432d2d5_25f4_4165_99c5_5935a7763c1a>
        <rdfs:comment>Subclasses of &apos;symbol&apos; are alphabets, in formal languages terminology.</rdfs:comment>
        <rdfs:comment>Symbols of a formal language need not be symbols of anything. For instance there are logical constants which do not refer to any idea, but rather serve as a form of punctuation in the language (e.g. parentheses). 

Symbols of a formal language must be capable of being specified without any reference to any interpretation of them. 
(Wikipedia)</rdfs:comment>
        <rdfs:comment>The class is the idea of the symbol, while the individual of that class stands for a specific mark (or token) of that idea.</rdfs:comment>
        <rdfs:label xml:lang="en">symbol</rdfs:label>
    </owl:Class>
    


    <!-- http://emmc.info/emmo-semiotics#EMMO_b21a56ed_f969_4612_a6ec_cb7766f7f31d -->

    <owl:Class rdf:about="http://emmc.info/emmo-semiotics#EMMO_b21a56ed_f969_4612_a6ec_cb7766f7f31d">
        <owl:equivalentClass>
            <owl:Class>
                <owl:unionOf rdf:parseType="Collection">
                    <rdf:Description rdf:about="http://emmc.info/emmo-semiotics#EMMO_0cd58641_824c_4851_907f_f4c3be76630c"/>
                    <rdf:Description rdf:about="http://emmc.info/emmo-semiotics#EMMO_35d2e130_6e01_41ed_94f7_00b333d46cf9"/>
                    <rdf:Description rdf:about="http://emmc.info/emmo-semiotics#EMMO_d7788d1a_020d_4c78_85a1_13563fcec168"/>
                </owl:unionOf>
            </owl:Class>
        </owl:equivalentClass>
        <rdfs:subClassOf rdf:resource="http://emmc.info/emmo-semiotics#EMMO_b803f122_4acb_4064_9d71_c1e5fd091fc9"/>
        <rdfs:subClassOf>
            <owl:Restriction>
                <owl:onProperty rdf:resource="http://emmc.info/emmo-core#EMMO_7afbed84_7593_4a23_bd88_9d9c6b04e8f6"/>
                <owl:allValuesFrom rdf:resource="http://emmc.info/emmo-semiotics#EMMO_b21a56ed_f969_4612_a6ec_cb7766f7f31d"/>
            </owl:Restriction>
        </rdfs:subClassOf>
        <emmo-core:EMMO_967080e5_2f42_4eb2_a3a9_c58143e835f9>An &apos;spacetime&apos; that is used as sign (&quot;semeion&quot; in greek) that stands for another &apos;spacetime&apos; through an semiotic process.</emmo-core:EMMO_967080e5_2f42_4eb2_a3a9_c58143e835f9>
        <emmo-core:EMMO_b432d2d5_25f4_4165_99c5_5935a7763c1a>A novel is made of chapters, paragraphs, sentences, words and characters (in a direct parthood mereological hierarchy). 

Each of them are &apos;sign&apos;-s. 

A character can be the a-tomistic &apos;sign&apos; for the class of texts.

The horizontal segment in the character &quot;A&quot; is direct part of &quot;A&quot; but it is not a &apos;sign&apos; itself.

For plain text we can propose the ASCII symbols, for math the fundamental math symbols.</emmo-core:EMMO_b432d2d5_25f4_4165_99c5_5935a7763c1a>
        <rdfs:comment>A &apos;sign&apos; can have temporal-direct-parts which are &apos;sign&apos; themselves.

A &apos;sign&apos; usually have &apos;sign&apos; spatial direct parts only up to a certain elementary semiotic level, in which the part is only a &apos;physical&apos; and no more a &apos;sign&apos; (i.e. it stands for nothing). This elementary semiotic level is peculiar to each particular system of signs (e.g. text, painting).

Just like an &apos;elementary&apos; in the &apos;physical&apos; branch, each &apos;sign&apos; branch should have an a-tomistic mereological part.</rdfs:comment>
        <rdfs:comment>According to Peirce, &apos;sign&apos; includes three subcategories:
- symbols: that stand for an object through convention
- indeces: that stand for an object due to causal continguity
- icon: that stand for an object due to similitudes e.g. in shape or composition</rdfs:comment>
        <rdfs:comment>In a 4D ontology one could question if a &apos;sign&apos; should be defined as a spatial direct part of a &apos;semiosis&apos; i.e. a proper part of a &apos;semiosis&apos; during all its existence.

e.g. one can say that an unread text is not a &apos;sign&apos;: it was a &apos;sign&apos; during the &apos;semiosis&apos; process in which it was written, but after that it is something else, until somebody read it again.

However, this is not the case for an ontology, since declaring an individual under the &apos;sign&apos; class (a semiosis outside the EMMO, a meta-semiosis) is equivalent to say that for the ontologist (an interpreter outside the EMMO, a meta-interpreter) the real entity (an object outside the EMMO, a meta-object) is a &apos;sign&apos;.

So the &apos;semiosis&apos; process within the EMMO is about how other &apos;interpreter&apos;-s deal with the &apos;sign&apos;-s here declared.</rdfs:comment>
        <rdfs:comment>It can be defined as the semiotic branch of the EMMO.

&apos;sign&apos; subclasses categorize the type of signs that are used to create representations/models of the real world entities.</rdfs:comment>
        <rdfs:label xml:lang="en">sign</rdfs:label>
    </owl:Class>
    


    <!-- http://emmc.info/emmo-semiotics#EMMO_b803f122_4acb_4064_9d71_c1e5fd091fc9 -->

    <owl:Class rdf:about="http://emmc.info/emmo-semiotics#EMMO_b803f122_4acb_4064_9d71_c1e5fd091fc9">
        <owl:equivalentClass>
            <owl:Class>
                <owl:unionOf rdf:parseType="Collection">
                    <rdf:Description rdf:about="http://emmc.info/emmo-semiotics#EMMO_0527413c_b286_4e9c_b2d0_03fb2a038dee"/>
                    <rdf:Description rdf:about="http://emmc.info/emmo-semiotics#EMMO_6f5af708_f825_4feb_a0d1_a8d813d3022b"/>
                    <rdf:Description rdf:about="http://emmc.info/emmo-semiotics#EMMO_b21a56ed_f969_4612_a6ec_cb7766f7f31d"/>
                </owl:unionOf>
            </owl:Class>
        </owl:equivalentClass>
        <rdfs:subClassOf rdf:resource="http://emmc.info/emmo-process#EMMO_49804605_c0fe_4538_abda_f70ba1dc8a5d"/>
        <rdfs:subClassOf>
            <owl:Restriction>
                <owl:onProperty>
                    <rdf:Description>
                        <owl:inverseOf rdf:resource="http://emmc.info/emmo-process#EMMO_c5aae418_1622_4d02_93c5_21159e28e6c1"/>
                    </rdf:Description>
                </owl:onProperty>
                <owl:someValuesFrom rdf:resource="http://emmc.info/emmo-semiotics#EMMO_008fd3b2_4013_451f_8827_52bceab11841"/>
            </owl:Restriction>
        </rdfs:subClassOf>
        <emmo-core:EMMO_967080e5_2f42_4eb2_a3a9_c58143e835f9>The class of individuals that stands for semiotic objects, i.e. objects that take part on a semiotic process.</emmo-core:EMMO_967080e5_2f42_4eb2_a3a9_c58143e835f9>
        <rdfs:comment>Semiotic subclasse are defined using Peirce&apos;s semiotic theory.

&quot;Namely, a sign is something, A, which brings something, B, its interpretant sign determined or created by it, into the same sort of correspondence with something, C, its object, as that in which itself stands to C.&quot; (Peirce 1902, NEM 4, 20–21).

The triadic elements:
- &apos;sign&apos;: the sign A (e.g. a name)
- &apos;interpretant&apos;: the sign B as the effects of the sign A on the interpreter (e.g. the mental concept of what a name means)
- &apos;object&apos;: the object C (e.g. the entity to which the sign A and B refer to)

This class includes also the &apos;interpeter&apos; i.e. the entity that connects the &apos;sign&apos; to the &apos;object&apos;</rdfs:comment>
        <rdfs:label xml:lang="en">semiotic</rdfs:label>
    </owl:Class>
    


    <!-- http://emmc.info/emmo-semiotics#EMMO_c74da218_9147_4f03_92d1_8894abca55f3 -->

    <owl:Class rdf:about="http://emmc.info/emmo-semiotics#EMMO_c74da218_9147_4f03_92d1_8894abca55f3">
        <rdfs:subClassOf rdf:resource="http://emmc.info/emmo-core#EMMO_c5ddfdba_c074_4aa4_ad6b_1ac4942d300d"/>
        <emmo-core:EMMO_967080e5_2f42_4eb2_a3a9_c58143e835f9>A &apos;physical&apos; which stands for a real world object that is the result of the activity of an agent in the form of a spatial configuration of-the or within-the object, whose pattern is identifiable by an observer.</emmo-core:EMMO_967080e5_2f42_4eb2_a3a9_c58143e835f9>
        <rdfs:comment>From the Ancient Greek γραφή (graphḗ) which means drawing, painting, writing, a writing, description, and from γράφω (gráphō) which means scratch, carve.</rdfs:comment>
        <rdfs:label xml:lang="en">graphical</rdfs:label>
    </owl:Class>
    


    <!-- http://emmc.info/emmo-semiotics#EMMO_d7788d1a_020d_4c78_85a1_13563fcec168 -->

    <owl:Class rdf:about="http://emmc.info/emmo-semiotics#EMMO_d7788d1a_020d_4c78_85a1_13563fcec168">
        <rdfs:subClassOf rdf:resource="http://emmc.info/emmo-semiotics#EMMO_b21a56ed_f969_4612_a6ec_cb7766f7f31d"/>
        <emmo-core:EMMO_967080e5_2f42_4eb2_a3a9_c58143e835f9>A &apos;sign&apos; that stands for an &apos;object&apos; by resembling or imitating it, in shape or by sharing a similar logical structure.</emmo-core:EMMO_967080e5_2f42_4eb2_a3a9_c58143e835f9>
        <emmo-core:EMMO_b432d2d5_25f4_4165_99c5_5935a7763c1a>A picture that reproduces the aspect of a person. 

An equation that reproduces the logical connection of the properties of a physical entity.</emmo-core:EMMO_b432d2d5_25f4_4165_99c5_5935a7763c1a>
        <rdfs:label xml:lang="en">icon</rdfs:label>
    </owl:Class>
    


    <!-- 
    ///////////////////////////////////////////////////////////////////////////////////////
    //
    // Individuals
    //
    ///////////////////////////////////////////////////////////////////////////////////////
     -->

    


    <!-- http://emmc.info/emmo-core#EMMO_08cb807c_e626_447b_863f_e2835540e918 -->

    <owl:NamedIndividual rdf:about="http://emmc.info/emmo-core#EMMO_08cb807c_e626_447b_863f_e2835540e918">
        <rdf:type rdf:resource="http://emmc.info/emmo-core#EMMO_802d3e92_8770_4f98_a289_ccaaab7fdddf"/>
        <rdf:type rdf:resource="http://emmc.info/emmo-core#EMMO_c5ddfdba_c074_4aa4_ad6b_1ac4942d300d"/>
        <rdf:type rdf:resource="http://emmc.info/emmo-core#EMMO_eb3a768e_d53e_4be9_a23b_0714833c36de"/>
        <rdfs:label xml:lang="en">universe</rdfs:label>
    </owl:NamedIndividual>
    


    <!-- http://emmc.info/emmo-granularity#EMMO_08f4d577_c604_4edd_9f29_d01e2da3a357 -->

    <owl:NamedIndividual rdf:about="http://emmc.info/emmo-granularity#EMMO_08f4d577_c604_4edd_9f29_d01e2da3a357">
        <rdf:type rdf:resource="http://emmc.info/emmo-core#EMMO_802d3e92_8770_4f98_a289_ccaaab7fdddf"/>
        <rdf:type rdf:resource="http://emmc.info/emmo-core#EMMO_c5ddfdba_c074_4aa4_ad6b_1ac4942d300d"/>
        <rdf:type rdf:resource="http://emmc.info/emmo-core#EMMO_eb3a768e_d53e_4be9_a23b_0714833c36de"/>
        <rdf:type rdf:resource="http://emmc.info/emmo-granularity#EMMO_36c79456_e29c_400d_8bd3_0eedddb82652"/>
        <rdf:type rdf:resource="http://emmc.info/emmo-granularity#EMMO_52211e5e_d767_4812_845e_eb6b402c476a"/>
        <rdfs:label xml:lang="en">a_1</rdfs:label>
    </owl:NamedIndividual>
    


    <!-- http://emmc.info/emmo-granularity#EMMO_0d68010b_56c1_4eb0_b569_9168965eee21 -->

    <owl:NamedIndividual rdf:about="http://emmc.info/emmo-granularity#EMMO_0d68010b_56c1_4eb0_b569_9168965eee21">
        <rdf:type rdf:resource="http://emmc.info/emmo-core#EMMO_802d3e92_8770_4f98_a289_ccaaab7fdddf"/>
        <rdf:type rdf:resource="http://emmc.info/emmo-core#EMMO_c5ddfdba_c074_4aa4_ad6b_1ac4942d300d"/>
        <rdf:type rdf:resource="http://emmc.info/emmo-core#EMMO_eb3a768e_d53e_4be9_a23b_0714833c36de"/>
        <rdf:type rdf:resource="http://emmc.info/emmo-granularity#EMMO_52211e5e_d767_4812_845e_eb6b402c476a"/>
        <rdfs:label xml:lang="en">b</rdfs:label>
    </owl:NamedIndividual>
    


    <!-- http://emmc.info/emmo-granularity#EMMO_7485aa48_9486_41ee_8b3d_85e6b284d6a7 -->

    <owl:NamedIndividual rdf:about="http://emmc.info/emmo-granularity#EMMO_7485aa48_9486_41ee_8b3d_85e6b284d6a7">
        <rdf:type rdf:resource="http://emmc.info/emmo-core#EMMO_802d3e92_8770_4f98_a289_ccaaab7fdddf"/>
        <rdf:type rdf:resource="http://emmc.info/emmo-core#EMMO_c5ddfdba_c074_4aa4_ad6b_1ac4942d300d"/>
        <rdf:type rdf:resource="http://emmc.info/emmo-core#EMMO_eb3a768e_d53e_4be9_a23b_0714833c36de"/>
        <rdf:type rdf:resource="http://emmc.info/emmo-granularity#EMMO_36c79456_e29c_400d_8bd3_0eedddb82652"/>
        <rdf:type rdf:resource="http://emmc.info/emmo-granularity#EMMO_52211e5e_d767_4812_845e_eb6b402c476a"/>
        <rdfs:label xml:lang="en">a_0</rdfs:label>
    </owl:NamedIndividual>
    


    <!-- http://emmc.info/emmo-granularity#EMMO_9517d355_bf61_427d_87fb_d5a38e7ee29a -->

    <owl:NamedIndividual rdf:about="http://emmc.info/emmo-granularity#EMMO_9517d355_bf61_427d_87fb_d5a38e7ee29a">
        <rdf:type rdf:resource="http://emmc.info/emmo-core#EMMO_802d3e92_8770_4f98_a289_ccaaab7fdddf"/>
        <rdf:type rdf:resource="http://emmc.info/emmo-core#EMMO_c5ddfdba_c074_4aa4_ad6b_1ac4942d300d"/>
        <rdf:type rdf:resource="http://emmc.info/emmo-core#EMMO_eb3a768e_d53e_4be9_a23b_0714833c36de"/>
        <rdf:type rdf:resource="http://emmc.info/emmo-granularity#EMMO_52211e5e_d767_4812_845e_eb6b402c476a"/>
        <emmo-granularity:EMMO_65a2c5b8_e4d8_4a51_b2f8_e55effc0547d rdf:resource="http://emmc.info/emmo-granularity#EMMO_da23c642_55b8_4835_b7b3_69da9155b31e"/>
        <emmo-granularity:EMMO_65a2c5b8_e4d8_4a51_b2f8_e55effc0547d rdf:resource="http://emmc.info/emmo-granularity#EMMO_ede401a8_91b9_43ba_ac9f_edc754df23eb"/>
        <emmo-granularity:EMMO_b2282816_b7a3_44c6_b2cb_3feff1ceb7fe rdf:resource="http://emmc.info/emmo-granularity#EMMO_ce487e67_a59c_40df_a8fc_fcc9f53bf029"/>
        <rdfs:label xml:lang="en">c</rdfs:label>
    </owl:NamedIndividual>
    


    <!-- http://emmc.info/emmo-granularity#EMMO_ce487e67_a59c_40df_a8fc_fcc9f53bf029 -->

    <owl:NamedIndividual rdf:about="http://emmc.info/emmo-granularity#EMMO_ce487e67_a59c_40df_a8fc_fcc9f53bf029">
        <rdf:type rdf:resource="http://emmc.info/emmo-core#EMMO_802d3e92_8770_4f98_a289_ccaaab7fdddf"/>
        <rdf:type rdf:resource="http://emmc.info/emmo-core#EMMO_c5ddfdba_c074_4aa4_ad6b_1ac4942d300d"/>
        <rdf:type rdf:resource="http://emmc.info/emmo-core#EMMO_eb3a768e_d53e_4be9_a23b_0714833c36de"/>
        <rdf:type rdf:resource="http://emmc.info/emmo-granularity#EMMO_52211e5e_d767_4812_845e_eb6b402c476a"/>
        <emmo-granularity:EMMO_65a2c5b8_e4d8_4a51_b2f8_e55effc0547d rdf:resource="http://emmc.info/emmo-granularity#EMMO_08f4d577_c604_4edd_9f29_d01e2da3a357"/>
        <emmo-granularity:EMMO_65a2c5b8_e4d8_4a51_b2f8_e55effc0547d rdf:resource="http://emmc.info/emmo-granularity#EMMO_7485aa48_9486_41ee_8b3d_85e6b284d6a7"/>
        <rdfs:label xml:lang="en">a</rdfs:label>
    </owl:NamedIndividual>
    


    <!-- http://emmc.info/emmo-granularity#EMMO_da23c642_55b8_4835_b7b3_69da9155b31e -->

    <owl:NamedIndividual rdf:about="http://emmc.info/emmo-granularity#EMMO_da23c642_55b8_4835_b7b3_69da9155b31e">
        <rdf:type rdf:resource="http://emmc.info/emmo-core#EMMO_802d3e92_8770_4f98_a289_ccaaab7fdddf"/>
        <rdf:type rdf:resource="http://emmc.info/emmo-core#EMMO_c5ddfdba_c074_4aa4_ad6b_1ac4942d300d"/>
        <rdf:type rdf:resource="http://emmc.info/emmo-core#EMMO_eb3a768e_d53e_4be9_a23b_0714833c36de"/>
        <rdf:type rdf:resource="http://emmc.info/emmo-granularity#EMMO_36c79456_e29c_400d_8bd3_0eedddb82652"/>
        <rdf:type rdf:resource="http://emmc.info/emmo-granularity#EMMO_52211e5e_d767_4812_845e_eb6b402c476a"/>
        <emmo-granularity:EMMO_b2282816_b7a3_44c6_b2cb_3feff1ceb7fe rdf:resource="http://emmc.info/emmo-granularity#EMMO_08f4d577_c604_4edd_9f29_d01e2da3a357"/>
        <rdfs:label xml:lang="en">c_1</rdfs:label>
    </owl:NamedIndividual>
    


    <!-- http://emmc.info/emmo-granularity#EMMO_ede401a8_91b9_43ba_ac9f_edc754df23eb -->

    <owl:NamedIndividual rdf:about="http://emmc.info/emmo-granularity#EMMO_ede401a8_91b9_43ba_ac9f_edc754df23eb">
        <rdf:type rdf:resource="http://emmc.info/emmo-core#EMMO_802d3e92_8770_4f98_a289_ccaaab7fdddf"/>
        <rdf:type rdf:resource="http://emmc.info/emmo-core#EMMO_c5ddfdba_c074_4aa4_ad6b_1ac4942d300d"/>
        <rdf:type rdf:resource="http://emmc.info/emmo-core#EMMO_eb3a768e_d53e_4be9_a23b_0714833c36de"/>
        <rdf:type rdf:resource="http://emmc.info/emmo-granularity#EMMO_36c79456_e29c_400d_8bd3_0eedddb82652"/>
        <rdf:type rdf:resource="http://emmc.info/emmo-granularity#EMMO_52211e5e_d767_4812_845e_eb6b402c476a"/>
        <emmo-granularity:EMMO_b2282816_b7a3_44c6_b2cb_3feff1ceb7fe rdf:resource="http://emmc.info/emmo-granularity#EMMO_0d68010b_56c1_4eb0_b569_9168965eee21"/>
        <emmo-granularity:EMMO_b2282816_b7a3_44c6_b2cb_3feff1ceb7fe rdf:resource="http://emmc.info/emmo-granularity#EMMO_7485aa48_9486_41ee_8b3d_85e6b284d6a7"/>
        <rdfs:label xml:lang="en">c_0</rdfs:label>
    </owl:NamedIndividual>
    


    <!-- 
    ///////////////////////////////////////////////////////////////////////////////////////
    //
    // Annotations
    //
    ///////////////////////////////////////////////////////////////////////////////////////
     -->

    <rdf:Description rdf:about="http://emmc.info/emmo-core#EMMO_548343f9_4257_47fe_aaab_488587ed41f0">
        <emmo-core:EMMO_967080e5_2f42_4eb2_a3a9_c58143e835f9>A proper part that extends along the whole spatial dimension of an hybrid.</emmo-core:EMMO_967080e5_2f42_4eb2_a3a9_c58143e835f9>
    </rdf:Description>
    <rdf:Description rdf:about="http://emmc.info/emmo-core#EMMO_7bb33ab7_cc3e_418d_a57c_97651533c865">
        <emmo-core:EMMO_967080e5_2f42_4eb2_a3a9_c58143e835f9>A proper part that extends along the whole temporal dimension of an hybrid.</emmo-core:EMMO_967080e5_2f42_4eb2_a3a9_c58143e835f9>
    </rdf:Description>
    <rdf:Description rdf:about="http://www.w3.org/2002/07/owl#Thing">
        <rdfs:comment>A word between apices represents an OWL-DL class (e.g. &apos;emmo&apos;).</rdfs:comment>
        <rdfs:comment>In the following classes annotations we will often shorten expressions like:

- an individual of class &apos;my_class&apos;
- individuals of class &apos;my_class&apos;

with the expressions:

- a &apos;my_class&apos;
- some &apos;my_class&apos;</rdfs:comment>
    </rdf:Description>
</rdf:RDF>



<!-- Generated by the OWL API (version 4.2.8.20170104-2310) https://github.com/owlcs/owlapi -->

